viper-total-heaps/TotalSemanticsProperties.thy
@@ -963,6 +963,780 @@ qed
 
 
 
+subsection \<open>External Consistent State \<Longrightarrow> Inhaled State\<close>
+
+
+lemma extcons_state_can_be_inhaled_assertion:
+  assumes Sat: "sat ctxt \<omega>\<^sub>0 mh mp A"
+      and mh_nm: "mh = get_mh_nm nm"
+      and mp_nm: "mp = get_mp_nm nm"
+      and ExtCons: "consistent_external ctxt \<lparr> get_hh_total = hh, get_nm_total = nm \<rparr>"
+      and \<omega>hh: "get_hh_total_full \<omega> = hh"
+      and \<omega>\<^sub>0hh: "get_hh_total_full \<omega>\<^sub>0 = hh"
+      and SameStore: "get_store_total \<omega> = get_store_total \<omega>\<^sub>0"
+      and Framed: "assertion_framing_state ctxt StateCons A \<omega>"
+      and SupPred: "supported_pred_body A"
+      and FinalIntCons: "StateCons (add_to_nm_total_full \<omega> nm)"
+      and MonoCons: "mono_prop_downward StateCons"
+      and WfCtxt: "ctxt_pred_syn_wf ctxt"
+    shows "red_inhale ctxt StateCons A \<omega> (RNormal (add_to_nm_total_full \<omega> nm))"
+
+  using Sat mh_nm mp_nm ExtCons \<omega>hh SameStore Framed SupPred FinalIntCons
+proof (induction A arbitrary: \<omega> nm)
+
+  case IH: (SatAcc e_r r e_p p a mh f mp)
+  hence "supported_pred_expr e_r" and "supported_pred_expr e_p"
+    by simp+
+
+  obtain r_r where "ctxt, Some \<omega> \<turnstile> \<langle>e_r;\<omega>\<rangle> [\<Down>]\<^sub>t r_r"
+    by (metis IH.hyps(1) IH.prems(4) IH.prems(5) \<omega>\<^sub>0hh \<open>supported_pred_expr e_r\<close> eval_ok_no_type_error(1))
+  obtain r_p where "ctxt, Some \<omega> \<turnstile> \<langle>e_p;\<omega>\<rangle> [\<Down>]\<^sub>t r_p"
+    by (metis IH.hyps(2) IH.prems(4) IH.prems(5) \<omega>\<^sub>0hh \<open>supported_pred_expr e_p\<close> eval_ok_no_type_error(1))
+
+  have "\<And>res. ctxt, Some \<omega> \<turnstile> \<langle>e_r;\<omega>\<rangle> [\<Down>]\<^sub>t res \<Longrightarrow> res \<noteq> VFailure"
+    using IH.prems(6) RedExpListFailure assertion_framing_state_sub_exps_not_failure
+    by fastforce
+  hence eval_e_r: "ctxt, Some \<omega> \<turnstile> \<langle>e_r;\<omega>\<rangle> [\<Down>]\<^sub>t Val (VRef r)"
+    by (metis IH.hyps(1) IH.prems(4) IH.prems(5) \<omega>\<^sub>0hh \<open>ctxt, Some \<omega> \<turnstile> \<langle>e_r;\<omega>\<rangle> [\<Down>]\<^sub>t r_r\<close> \<open>supported_pred_expr e_r\<close> eval_with_same_store_same_hh(1) extended_val.exhaust_sel)
+
+  have "\<And>res. ctxt, Some \<omega> \<turnstile> \<langle>e_p;\<omega>\<rangle> [\<Down>]\<^sub>t res \<Longrightarrow> res \<noteq> VFailure"
+    using IH.prems(6) RedExpListCons RedExpListFailure assertion_framing_state_sub_exps_not_failure eval_e_r red_pure_exps_total.simps
+    by fastforce
+
+  hence eval_e_p: "ctxt, Some \<omega> \<turnstile> \<langle>e_p;\<omega>\<rangle> [\<Down>]\<^sub>t Val (VPerm p)"
+    by (metis IH(2) IH.prems(4) IH.prems(5) \<omega>\<^sub>0hh \<open>\<And>thesis. (\<And>r_p. ctxt, Some \<omega> \<turnstile> \<langle>e_p;\<omega>\<rangle> [\<Down>]\<^sub>t r_p \<Longrightarrow> thesis) \<Longrightarrow> thesis\<close> \<open>supported_pred_expr e_p\<close> eval_with_same_store_same_hh(1) extended_val.exhaust)
+
+  define W where "W = (if r = Null
+                       then {\<omega>}
+                       else inhale_perm_single StateCons \<omega> (the_address r, f) (Some (Abs_preal p)))"
+
+  show ?case
+    apply standard
+    using eval_e_r eval_e_p W_def
+       apply blast+
+  proof (cases "r = Null")
+    case True
+    with IH have "p = 0"
+      by presburger
+    from True W_def have "W = {\<omega>}"
+      by auto
+    have "nm = 0"
+      apply (rule nested_mask_equality)
+        apply (simp_all add: zero_nested_mask_def)
+      using IH.hyps(5) IH.prems(1) True
+        apply auto[1]
+      using IH.hyps(6) IH.prems(2)
+        apply auto[1]
+      using zero_mask_def
+      by (metis (no_types, lifting) Rep_posreal comp_apply mem_Collect_eq option.exhaust_sel option_fold.simps(1) pperm_pgt_pnone)
+    show "th_result_rel (0 \<le> p) (W \<noteq> {} \<and> (0 < p \<longrightarrow> r \<noteq> Null)) W (RNormal (add_to_nm_total_full \<omega> nm))"
+      apply (simp add: \<open>p = 0\<close> \<open>W = {\<omega>}\<close> True th_result_rel.simps)
+      by (simp add: zero_nested_mask_def[symmetric] \<open>nm = 0\<close>)
+  next
+    case False
+    have mh: "get_mh_nm nm = singleton_mh (a, f) (Abs_preal p)"
+      using False IH.hyps(5) IH.prems(1) by presburger
+    have fnm: "get_fnm_nm nm = (\<lambda>_. None)"
+      by (metis (mono_tags, lifting) IH.hyps(6) IH.prems(2) Rep_posreal comp_eq_dest_lhs get_mp_nm.simps mem_Collect_eq option.exhaust_sel option_fold.simps(1) preal_not_0_gt_0 zero_mask_def)
+    have intcons: "StateCons (upd_mh_loc_total_full \<omega> (the_address r, f) (get_mh_total_full \<omega> (the_address r, f) + Abs_preal p))"
+    proof -
+      have "upd_mh_loc_total_full \<omega> (the_address r, f) (get_mh_total_full \<omega> (the_address r, f) + Abs_preal p) =
+            add_to_nm_total_full \<omega> nm"
+        apply (rule full_total_state.equality; simp_all)
+        apply (rule total_state.equality; simp_all)
+        apply (rule nested_mask_equality; standard; simp add: add_masks_def)
+         apply (simp add: mh IH(3))
+        unfolding plus_nested_mask_def
+        apply (cases "get_nm_total_full \<omega>", cases nm)
+        apply simp
+        by (metis (no_types, lifting) combine_options_simps(2) fnm get_fnm_nm.simps pfun_comb_def)
+      thus ?thesis
+        using IH.prems(8) by presburger
+    qed
+    show "th_result_rel (0 \<le> p) (W \<noteq> {} \<and> (0 < p \<longrightarrow> r \<noteq> Null)) W (RNormal (add_to_nm_total_full \<omega> nm))"
+      apply (simp add: IH(4) W_def inhale_perm_single_def False intcons[simplified])
+      apply (rule THResultNormal)
+      apply (rule Set.CollectI)
+      apply (intro conjI)
+       apply (rule full_total_state.equality)
+          apply simp_all
+       apply (rule total_state.equality)
+         apply simp_all
+       apply (rule nested_mask_equality)
+        apply simp_all
+        apply (simp add: mh)
+        apply standard
+        apply simp
+        apply (simp add: IH.hyps(3) add_masks_def)
+      unfolding plus_nested_mask_def
+       apply (cases "get_nm_total_full \<omega>", cases nm)
+       apply standard
+       apply (simp add: pfun_comb_def)
+      using fnm
+       apply fastforce
+      by (metis IH.prems(8) add_to_nm_total.elims add_to_nm_total_full.simps plus_nested_mask_def)
+  qed
+
+next
+  case IH: (SatAccWildcard e_r r a f mh mp)
+
+  hence e_r_sup: "supported_pred_expr e_r"
+    by auto
+  obtain r_r where "ctxt, Some \<omega> \<turnstile> \<langle>e_r;\<omega>\<rangle> [\<Down>]\<^sub>t r_r"
+    using eval_ok_no_type_error(1) IH(1,9,10) \<omega>\<^sub>0hh e_r_sup
+    by metis
+  moreover have "\<And>res. ctxt, Some \<omega> \<turnstile> \<langle>e_r;\<omega>\<rangle> [\<Down>]\<^sub>t res \<Longrightarrow> res \<noteq> VFailure"
+    using IH.prems(6) RedExpListFailure assertion_framing_state_sub_exps_not_failure
+    by fastforce
+  ultimately have e_r_eval: "ctxt, Some \<omega> \<turnstile> \<langle>e_r;\<omega>\<rangle> [\<Down>]\<^sub>t Val (VRef r)"
+    by (metis IH.hyps(1) IH.prems(4) IH.prems(5) \<omega>\<^sub>0hh e_r_sup eval_with_same_store_same_hh(1) extended_val.exhaust)
+
+  define W where "W = inhale_perm_single StateCons \<omega> (the_address r, f) None"
+
+  have "is_singleton_mh (a,f) (get_mh_nm nm)"
+    using IH.hyps(4) IH.prems(1)
+    by auto
+  have "get_mp_nm nm = zero_mask"
+    using IH.hyps(5) IH.prems(2)
+    by presburger
+  hence "get_fnm_nm nm = (\<lambda>_. None)"
+    using SatAll_case[OF IH(8)]
+    by (metis (mono_tags, lifting) Rep_posreal comp_eq_dest_lhs get_mp_nm.simps mem_Collect_eq option.exhaust option_fold.simps(1) preal_not_0_gt_0 zero_mask_def)
+
+  have "add_to_nm_total_full \<omega> nm \<in> W"
+    apply (simp add: W_def inhale_perm_single_def)
+    apply (rule exI[of _ "get_mh_nm nm (a,f)"])
+    apply (intro conjI)
+    using \<open>is_singleton_mh (a, f) (get_mh_nm nm)\<close>
+       apply fastforce
+     apply (rule full_total_state.equality, simp_all)
+     apply (rule total_state.equality, simp_all)
+     apply (rule nested_mask_equality, simp_all; standard)
+      apply (simp_all add: add_masks_def)
+    using IH.hyps(2) \<open>is_singleton_mh (a, f) (get_mh_nm nm)\<close>
+      apply force
+    unfolding plus_nested_mask_def
+     apply (cases "get_nm_total_full \<omega>", cases nm)
+     apply (simp add: pfun_comb_def)
+    using \<open>get_fnm_nm nm = (\<lambda>_. None)\<close>
+     apply auto[1]
+    by (metis IH.prems(8) add_to_nm_total.elims add_to_nm_total_full.simps plus_nested_mask_def)
+  hence "W \<noteq> {}"
+    by fast
+
+  show ?case
+    apply (rule InhAccWildcard[where ?W'=W])
+    using e_r_eval
+      apply simp
+    using W_def
+     apply force
+    using IH.hyps(3) THResultNormal \<open>W \<noteq> {}\<close> \<open>add_to_nm_total_full \<omega> nm \<in> W\<close>
+    by auto
+
+next
+  case IH: (SatAccPred e_args v_args e_p p mh mp pred_id pred_decl)
+
+  hence e_args_sup: "list_all supported_pred_expr e_args" and
+        e_p_sup: "supported_pred_expr e_p"
+    by (simp add: list_all_length)+
+  then obtain r_vs r_p where
+    e_args_res: "red_pure_exps_total ctxt (Some \<omega>) e_args \<omega> r_vs" and
+    e_p_res: "ctxt, Some \<omega> \<turnstile> \<langle>e_p;\<omega>\<rangle> [\<Down>]\<^sub>t r_p"
+    using eval_ok_no_type_error IH(1,2,9,10) \<omega>\<^sub>0hh
+    by (metis (full_types) IH.prems(4) IH.prems(5))
+  have e_args_ok: "\<And>res. red_pure_exps_total ctxt (Some \<omega>) e_args \<omega> res \<Longrightarrow> res \<noteq> None" and
+          e_p_ok: "\<And>res. ctxt, Some \<omega> \<turnstile> \<langle>e_p;\<omega>\<rangle> [\<Down>]\<^sub>t res \<Longrightarrow> res \<noteq> VFailure"
+     apply (metis IH.prems(6) assertion_framing_state_sub_exps_not_failure red_pure_exps_total_append_failure sub_expressions_atomic.simps(3))
+    by (metis IH.prems(6) RedExpListFailure e_args_res assertion_framing_state_sub_exps_not_failure red_pure_exps_total_append_failure red_pure_exps_total_append_failure_2 split_option_ex sub_expressions_atomic.simps(3) sub_expressions_exp_or_wildcard.simps(1))
+  have e_args_eval: "red_pure_exps_total ctxt (Some \<omega>) e_args \<omega> (Some v_args)" and
+          e_p_eval: "ctxt, Some \<omega> \<turnstile> \<langle>e_p;\<omega>\<rangle> [\<Down>]\<^sub>t Val (VPerm p)"
+    using IH(1) eval_with_same_store_same_hh(2)[OF IH(1)]
+    apply (metis IH.prems(4) IH.prems(5) \<omega>\<^sub>0hh e_args_sup not_Some_eq e_args_ok e_args_res)
+    by (metis IH(2) IH.prems(4) IH.prems(5) \<omega>\<^sub>0hh e_p_res e_p_ok e_p_sup eval_with_same_store_same_hh(1) extended_val.exhaust)
+
+  define W where "W = inhale_perm_single_pred ctxt StateCons \<omega> (pred_id,v_args) (Some (Abs_preal p))"
+
+  have "get_mh_nm nm = zero_mask"
+    using IH.hyps(4) IH.prems(1)
+    by auto
+  have "get_mp_nm nm = singleton_mp (pred_id,v_args) (Abs_preal p)"
+    using IH.hyps(5) IH.prems(2)
+    by order
+  hence "get_mp_nm nm (pred_id,v_args) = Abs_preal p"
+    by simp
+
+  have sat: "sat ctxt \<omega>\<^sub>0 mh mp (Atomic (AccPredicate pred_id e_args (PureExp e_p)))"
+    using IH
+    by (meson SatAccPred)
+
+  obtain nm_pred where
+    p_nonzero: "p > 0 \<longrightarrow> get_fnm_nm nm (pred_id,v_args) = Some (Abs_posreal (Abs_preal p), nm_pred)" and
+    p_zero: "p = 0 \<longrightarrow> nm_pred = 0"
+    using \<open>get_mp_nm nm = _\<close>[THEN fun_cong, of "(pred_id,v_args)", simplified]
+    apply (cases "get_fnm_nm nm (pred_id,v_args)"; simp)
+    using positive_real_preal
+     apply blast
+    by (metis Rep_posreal_inverse fstI order_less_irrefl surj_pair)
+
+  have nm_pred_extcons: "consistent_external_wrt_ploc ctxt \<lparr> get_hh_total = hh, get_nm_total = nm_pred \<rparr> (pred_id,v_args) (Abs_preal p)"
+    apply (cases "p > 0")
+     apply (metis IH.prems(3) SatAll_case \<open>get_mp_nm nm (pred_id, v_args) = Abs_preal p\<close> comp_apply get_mp_nm.simps old.prod.inject option_fold.simps(1) p_nonzero prod.collapse total_state.select_convs(2) total_state.update_convs(2))
+    apply (subgoal_tac "p = 0")
+     prefer 2
+    using IH.hyps(3)
+     apply fastforce
+    apply (thin_tac _)
+    apply (rule SatStep)
+         apply (rule IH(6))
+        apply (rule IH(7))
+       apply (rule IH(8))
+      apply (simp add: p_zero)
+     apply (simp add: zero_preal_def)
+    by (simp add: empty_consistent_external p_zero)
+
+  have "p = 0 \<Longrightarrow> nm = 0"
+    apply (rule nested_mask_equality)
+     apply (simp add: \<open>get_mh_nm nm = zero_mask\<close> zero_nested_mask_def)
+    apply standard
+    apply (rename_tac lp)
+    apply (cut_tac ?x=lp in \<open>get_mp_nm nm = _\<close>[THEN fun_cong])
+    apply (case_tac "get_fnm_nm nm lp"; simp add: zero_nested_mask_def)
+    by (metis Rep_posreal mem_Collect_eq pperm_pgt_pnone zero_preal.abs_eq)
+
+  have "Abs_preal p \<noteq> 0 \<Longrightarrow> nm = NM zero_mask [(pred_id,v_args) \<mapsto> (Abs_posreal (Abs_preal p), nm_pred)]"
+    apply (rule nested_mask_equality)
+     apply (simp add: \<open>get_mh_nm nm = zero_mask\<close> zero_nested_mask_def)
+    apply standard
+    apply (rename_tac lp)
+    apply (cut_tac ?x=lp in \<open>get_mp_nm nm = _\<close>[THEN fun_cong])
+    apply (case_tac "get_fnm_nm nm lp")
+     apply fastforce
+    using IH.hyps(3) Rep_posreal map_upd_Some_unfold mem_Collect_eq option_fold.simps(1) p_nonzero pperm_pgt_pnone zero_preal.abs_eq
+    by fastforce
+
+  have "add_to_nm_total_full \<omega> nm \<in> W"
+    unfolding W_def inhale_perm_single_pred_def option_fold.simps
+    apply (rule CollectI)
+    apply simp
+    apply (rule exI[of _ "\<lparr> get_hh_total = hh, get_nm_total = nm_pred \<rparr>"])
+    apply (intro conjI)
+     apply (intro impI)
+     apply (intro conjI)
+    using nm_pred_extcons
+        apply auto[1]
+    using IH.prems(4)
+       apply auto[1]
+      apply (rule full_total_state.equality; simp)
+      apply (rule total_state.equality; simp)
+    using IH.hyps(3) \<open>p = 0 \<Longrightarrow> nm = 0\<close> positive_real_preal
+      apply fastforce
+    using IH.prems(8)
+     apply auto[1]
+    apply (intro impI)
+    apply (intro conjI)
+    using nm_pred_extcons IH.hyps(3) zero_preal.abs_eq
+       apply fastforce
+    using IH.prems(4)
+      apply auto[1]
+     apply (rule full_total_state.equality; simp)
+     apply (rule total_state.equality; simp)
+     apply (rule nested_mask_equality; simp)
+      apply (simp add: \<open>get_mh_nm nm = zero_mask\<close> add_masks_zero_mask)
+    using \<open>Abs_preal p \<noteq> 0 \<Longrightarrow> _\<close>
+     apply simp
+     apply standard
+     apply (rename_tac lp)
+     apply (cases "get_nm_total_full \<omega>", simp)
+     apply (rename_tac mh fnm)
+    unfolding plus_nested_mask_def
+     apply simp
+     apply (case_tac "lp = (pred_id,v_args)"; case_tac "fnm lp"; simp add: pfun_comb_def)
+    by (metis IH.prems(8) add_to_nm_total.elims add_to_nm_total_full.simps plus_nested_mask_def)
+
+  show ?case
+    apply (rule InhAccPred[where ?W'=W])
+    using e_args_eval e_p_eval
+       apply simp+
+    using W_def
+     apply force
+    using IH.hyps(3) THResultNormal \<open>add_to_nm_total_full \<omega> nm \<in> W\<close>
+    by (metis (full_types) empty_iff)
+
+next
+  case IH: (SatAccPredWildcard e_args v_args mh pred_id mp)
+
+  hence e_args_sup: "list_all supported_pred_expr e_args"
+    by (simp add: list_all_length)
+  then obtain r_vs where
+    e_args_res: "red_pure_exps_total ctxt (Some \<omega>) e_args \<omega> r_vs"
+    using eval_ok_no_type_error(2) IH(1,7,8,10) \<omega>\<^sub>0hh
+    by (metis (full_types) IH.prems(5))
+  have e_args_ok: "\<And>res. red_pure_exps_total ctxt (Some \<omega>) e_args \<omega> res \<Longrightarrow> res \<noteq> None"
+    by (metis IH.prems(6) assertion_framing_state_sub_exps_not_failure red_pure_exps_total_append_failure sub_expressions_atomic.simps(3))
+  have e_args_eval: "red_pure_exps_total ctxt (Some \<omega>) e_args \<omega> (Some v_args)"
+    using IH(1) eval_with_same_store_same_hh(2)[OF IH(1)]
+    by (metis IH.prems(4) IH.prems(5) \<omega>\<^sub>0hh e_args_sup not_Some_eq e_args_ok e_args_res)
+
+  define W where "W = inhale_perm_single_pred ctxt StateCons \<omega> (pred_id,v_args) None"
+
+  have "get_mh_nm nm = zero_mask"
+    using IH.hyps(2) IH.prems(1)
+    by auto
+  have "is_singleton_mp (pred_id,v_args) (get_mp_nm nm)"
+    using IH.hyps(3) IH.prems(2)
+    by meson
+  then obtain p where p: "get_mp_nm nm = singleton_mp (pred_id,v_args) p" and "p > 0"
+    by auto
+
+  have sat: "sat ctxt \<omega>\<^sub>0 mh mp (Atomic (AccPredicate pred_id e_args Wildcard))"
+    using IH
+    by (meson SatAccPredWildcard)
+
+  obtain nm_pred where
+    p_nonzero: "p > 0 \<longrightarrow> get_fnm_nm nm (pred_id,v_args) = Some (Abs_posreal p, nm_pred)" and
+    p_zero: "p = 0 \<longrightarrow> nm_pred = 0"
+    using \<open>get_mp_nm nm = _\<close>[THEN fun_cong, of "(pred_id,v_args)", simplified]
+    apply (cases "get_fnm_nm nm (pred_id,v_args)"; simp)
+    by (metis Rep_posreal_inverse fstI order_less_irrefl surj_pair)
+
+  have nm_pred_extcons: "consistent_external_wrt_ploc ctxt \<lparr> get_hh_total = hh, get_nm_total = nm_pred \<rparr> (pred_id,v_args) p"
+    apply (cases "p > 0")
+     apply (metis IH.prems(3) SatAll_case mem_Collect_eq p_nonzero posreal_to_preal(8) total_state.select_convs(2) total_state.update_convs(2))
+    apply (subgoal_tac "p = 0")
+     prefer 2
+     apply (simp add: \<open>0 < p\<close>)
+    apply (thin_tac _)
+    apply (rule SatStep)
+         apply (rule IH(4))
+        apply (rule IH(5))
+       apply (rule IH(6))
+      apply (simp add: p_zero)
+     apply (simp add: zero_preal_def)
+    by (simp add: empty_consistent_external p_zero)
+
+  have "p \<noteq> 0 \<Longrightarrow> nm = NM zero_mask [(pred_id,v_args) \<mapsto> (Abs_posreal p, nm_pred)]"
+    apply (rule nested_mask_equality)
+     apply (simp add: \<open>get_mh_nm nm = zero_mask\<close> zero_nested_mask_def)
+    apply standard
+    apply (rename_tac lp)
+    apply (cut_tac ?x=lp in \<open>get_mp_nm nm = _\<close>[THEN fun_cong])
+    apply (case_tac "get_fnm_nm nm lp")
+     apply fastforce
+    using IH.hyps(3) Rep_posreal map_upd_Some_unfold mem_Collect_eq option_fold.simps(1) p_nonzero pperm_pgt_pnone zero_preal.abs_eq
+    by (metis (mono_tags, lifting) comp_apply get_fnm_nm.simps get_mp_nm.simps singleton_mp.elims)
+
+  have "add_to_nm_total_full \<omega> nm \<in> W"
+    unfolding W_def inhale_perm_single_pred_def option_fold.simps
+    apply (rule CollectI)
+    apply simp
+    apply (rule exI[of _ "\<lparr> get_hh_total = hh, get_nm_total = nm_pred \<rparr>"])
+    apply (rule exI[of _ p])
+    apply (intro conjI)
+    using \<open>pos_perm_class.pnone < p\<close>
+     apply force
+    apply (intro impI)
+    apply (intro conjI)
+    using nm_pred_extcons
+       apply presburger
+    using IH.prems(4)
+      apply auto[1]
+     apply (rule full_total_state.equality; simp)
+     apply (rule total_state.equality; simp)
+     apply (rule nested_mask_equality; simp)
+      apply (simp add: \<open>get_mh_nm nm = zero_mask\<close> add_masks_zero_mask)
+    using \<open>p \<noteq> 0 \<Longrightarrow> _\<close>
+     apply simp
+     apply standard
+     apply (rename_tac lp)
+     apply (cases "get_nm_total_full \<omega>", simp)
+     apply (rename_tac mh fnm)
+    unfolding plus_nested_mask_def
+     apply simp
+     apply (case_tac "lp = (pred_id,v_args)"; case_tac "fnm lp"; simp add: pfun_comb_def)
+    by (metis IH.prems(8) add_to_nm_total.elims add_to_nm_total_full.simps plus_nested_mask_def)
+
+  show ?case
+    apply (rule InhAccPredWildcard[where ?W'=W])
+    using e_args_eval
+      apply simp
+    using W_def
+     apply force
+    using IH.hyps(3) THResultNormal \<open>add_to_nm_total_full \<omega> nm \<in> W\<close>
+    by (metis (full_types) ex_in_conv)
+
+next
+  case IH: (SatPure e mh mp)
+  hence "supported_pred_expr e"
+    by simp
+  then obtain res where \<omega>_eval: "ctxt, Some \<omega> \<turnstile> \<langle>e;\<omega>\<rangle> [\<Down>]\<^sub>t res"
+    by (metis IH.hyps(1) IH.prems(4) IH.prems(5) eval_ok_no_type_error(1) \<omega>\<^sub>0hh)
+  show ?case
+  proof (cases res)
+    case (Val v)
+    then have "v = VBool True"
+      using eval_with_same_store_same_hh(1)[OF IH(1)] IH(10) IH(7) IH(8) \<omega>\<^sub>0hh \<omega>_eval \<open>supported_pred_expr e\<close>
+      apply simp
+      by presburger
+    have "nm = 0"
+      apply (rule nested_mask_equality)
+       apply (metis IH.hyps(2) IH.prems(1) zero_nested_mask_def get_mh_nm.simps)
+      apply (simp add: zero_nested_mask_def)
+      apply standard
+      using IH(5)
+      by (metis IH.hyps(3) get_mp_0_implies_fnm_None zero_mask_def)
+    hence "add_to_nm_total_full \<omega> nm = \<omega>"
+      by (simp add: zero_nested_mask_def[symmetric])
+    then show ?thesis
+      by (metis Val \<omega>_eval \<open>v = VBool True\<close> inh_pure_normal)
+  next
+    case VFailure
+    then show ?thesis
+      using IH.prems(6) RedExpListFailure \<omega>_eval assertion_framing_state_sub_exps_not_failure by fastforce
+  qed
+
+next
+  case IH: (SatStar mh mh\<^sub>1 mh\<^sub>2 mp mp\<^sub>1 mp\<^sub>2 A B)
+
+  hence A_sup: "supported_pred_body A" and B_sup: "supported_pred_body B"
+    by simp+
+
+  obtain fnm where fnm: "fnm = get_fnm_nm nm"
+    by simp
+  obtain fnm\<^sub>1 where fnm\<^sub>1: "\<And>lp. fnm\<^sub>1 lp = (if mp\<^sub>1 lp = 0 then None else Some (Abs_posreal (mp\<^sub>1 lp), (mp\<^sub>1 lp / mp lp) *\<^sub>s (snd (the (fnm lp)))))"
+    by simp
+  obtain fnm\<^sub>2 where fnm\<^sub>2: "\<And>lp. fnm\<^sub>2 lp = (if mp\<^sub>2 lp = 0 then None else Some (Abs_posreal (mp\<^sub>2 lp), (mp\<^sub>2 lp / mp lp) *\<^sub>s (snd (the (fnm lp)))))"
+    by simp
+  obtain nm\<^sub>1 where nm\<^sub>1: "nm\<^sub>1 = NM mh\<^sub>1 fnm\<^sub>1"
+    by simp
+  obtain nm\<^sub>2 where nm\<^sub>2: "nm\<^sub>2 = NM mh\<^sub>2 fnm\<^sub>2"
+    by simp
+
+  have "mp\<^sub>1 = get_mp_nm nm\<^sub>1"
+    unfolding nm\<^sub>1
+    apply simp
+    apply standard
+    apply (rename_tac lp)
+    apply (case_tac "fnm\<^sub>1 lp"; cut_tac ?lp=lp in fnm\<^sub>1; simp)
+     apply (metis option.distinct(1))
+    by (metis Abs_posreal_inverse Some_Some_ifD fst_eqD mem_Collect_eq option.inject pperm_pnone_pgt)
+  have "mp\<^sub>2 = get_mp_nm nm\<^sub>2"
+    unfolding nm\<^sub>2
+    apply simp
+    apply standard
+    apply (rename_tac lp)
+    apply (case_tac "fnm\<^sub>2 lp"; cut_tac ?lp=lp in fnm\<^sub>2; simp)
+     apply (metis option.distinct(1))
+    by (metis Abs_posreal_inverse Some_Some_ifD fst_eqD mem_Collect_eq option.inject pperm_pnone_pgt)
+
+  have nm\<^sub>1_cons: "consistent_external ctxt \<lparr> get_hh_total = hh, get_nm_total = nm\<^sub>1 \<rparr>"
+  proof
+    fix pid vs q nm'
+    assume lpm: "Some (q,nm') = get_fnm_total \<lparr> get_hh_total = hh, get_nm_total = nm\<^sub>1 \<rparr> (pid,vs)"
+    have "q = Abs_posreal (mp\<^sub>1 (pid,vs))" and
+         "nm' = (mp\<^sub>1 (pid,vs) / mp (pid,vs)) *\<^sub>s (snd (the (fnm (pid,vs))))"
+      using lpm[unfolded nm\<^sub>1, simplified, simplified fnm\<^sub>1]
+      by (cases "mp\<^sub>1 (pid,vs) = 0"; simp)+
+
+    have "mp (pid,vs) \<ge> mp\<^sub>1 (pid,vs)"
+      by (meson IH.hyps(2) le_funD split_implies_le(1))
+    then obtain q\<^sub>a nm'\<^sub>a where "Some (q\<^sub>a,nm'\<^sub>a) = get_fnm_total \<lparr> get_hh_total = hh, get_nm_total = nm \<rparr> (pid,vs)"
+      by (metis IH.prems(2) dual_order.strict_trans1 fnm\<^sub>1 get_fnm_nm.simps get_fnm_total.simps lpm nm\<^sub>1 obtain_lpm_from_mp option.distinct(1) preal_not_0_gt_0 total_state.select_convs(2))
+
+    hence extcons\<^sub>a: "consistent_external_wrt_ploc ctxt \<lparr> get_hh_total = hh, get_nm_total = nm'\<^sub>a \<rparr> (pid,vs) (Rep_posreal q\<^sub>a)"
+      by (metis IH.prems(3) consistent_external.cases total_state.update_convs(2))
+
+    have the_eq: "snd (the (fnm (pid,vs))) = nm'\<^sub>a"
+      by (metis \<open>Some (q\<^sub>a, nm'\<^sub>a) = _\<close> fnm get_fnm_total.simps option.sel sndI total_state.select_convs(2))
+
+    have q_pos: "mp\<^sub>1 (pid,vs) > 0"
+      using fnm\<^sub>1 lpm nm\<^sub>1 preal_not_0_gt_0
+      by fastforce
+
+    have "Rep_posreal q\<^sub>a = mp (pid,vs)"
+      by (metis Abs_posreal_inverse IH.prems(2) \<open>Some (q\<^sub>a, nm'\<^sub>a) = _\<close> \<open>mp\<^sub>1 (pid, vs) \<le> mp (pid, vs)\<close> dual_order.strict_trans1 fst_conv get_fnm_total.simps mem_Collect_eq obtain_lpm_from_mp option.sel q_pos total_state.select_convs(2))
+
+    show "consistent_external_wrt_ploc ctxt (\<lparr> get_hh_total = hh, get_nm_total = nm\<^sub>1 \<rparr>\<lparr> get_nm_total := nm' \<rparr>) (pid,vs) (Rep_posreal q)"
+      apply simp
+      unfolding \<open>nm' = _\<close> the_eq \<open>q = _\<close> Abs_posreal_inverse[of "mp\<^sub>1 (pid,vs)", simplified, OF q_pos]
+      using fraction_consistent_external(1)[OF WfCtxt extcons\<^sub>a, of "mp\<^sub>1 (pid, vs) / mp (pid, vs)", unfolded \<open>Rep_posreal q\<^sub>a = _\<close>, simplified]
+      by (metis (mono_tags, lifting) Rep_preal_inject \<open>mp\<^sub>1 (pid, vs) \<le> mp (pid, vs)\<close> divide_preal.rep_eq dual_order.strict_trans1 nonzero_eq_divide_eq pperm_pgt_pnone q_pos times_preal.rep_eq zero_preal.rep_eq)
+  qed
+
+  have nm\<^sub>2_cons: "consistent_external ctxt \<lparr> get_hh_total = hh, get_nm_total = nm\<^sub>2 \<rparr>"
+  proof
+    fix pid vs q nm'
+    assume lpm: "Some (q,nm') = get_fnm_total \<lparr> get_hh_total = hh, get_nm_total = nm\<^sub>2 \<rparr> (pid,vs)"
+    have "q = Abs_posreal (mp\<^sub>2 (pid,vs))" and
+         "nm' = (mp\<^sub>2 (pid,vs) / mp (pid,vs)) *\<^sub>s (snd (the (fnm (pid,vs))))"
+      using lpm[unfolded nm\<^sub>2, simplified, simplified fnm\<^sub>2]
+      by (cases "mp\<^sub>2 (pid,vs) = 0"; simp)+
+
+    have "mp (pid,vs) \<ge> mp\<^sub>2 (pid,vs)"
+      by (meson IH.hyps(2) le_funE split_implies_le(2))
+    then obtain q\<^sub>a nm'\<^sub>a where "Some (q\<^sub>a,nm'\<^sub>a) = get_fnm_total \<lparr> get_hh_total = hh, get_nm_total = nm \<rparr> (pid,vs)"
+      by (metis IH.prems(2) dual_order.strict_trans1 fnm\<^sub>2 get_fnm_nm.simps get_fnm_total.simps lpm nm\<^sub>2 obtain_lpm_from_mp option.distinct(1) preal_not_0_gt_0 total_state.select_convs(2))
+
+    hence extcons\<^sub>a: "consistent_external_wrt_ploc ctxt \<lparr> get_hh_total = hh, get_nm_total = nm'\<^sub>a \<rparr> (pid,vs) (Rep_posreal q\<^sub>a)"
+      by (metis IH.prems(3) consistent_external.cases total_state.update_convs(2))
+
+    have the_eq: "snd (the (fnm (pid,vs))) = nm'\<^sub>a"
+      by (metis \<open>Some (q\<^sub>a, nm'\<^sub>a) = _\<close> fnm get_fnm_total.simps option.sel sndI total_state.select_convs(2))
+
+    have q_pos: "mp\<^sub>2 (pid,vs) > 0"
+      using fnm\<^sub>2 lpm nm\<^sub>2 preal_not_0_gt_0
+      by fastforce
+
+    have "Rep_posreal q\<^sub>a = mp (pid,vs)"
+      by (metis Abs_posreal_inverse IH.prems(2) \<open>Some (q\<^sub>a, nm'\<^sub>a) = _\<close> \<open>mp\<^sub>2 (pid, vs) \<le> mp (pid, vs)\<close> dual_order.strict_trans1 fst_conv get_fnm_total.simps mem_Collect_eq obtain_lpm_from_mp option.sel q_pos total_state.select_convs(2))
+
+    show "consistent_external_wrt_ploc ctxt (\<lparr> get_hh_total = hh, get_nm_total = nm\<^sub>2 \<rparr>\<lparr> get_nm_total := nm' \<rparr>) (pid,vs) (Rep_posreal q)"
+      apply simp
+      unfolding \<open>nm' = _\<close> the_eq \<open>q = _\<close> Abs_posreal_inverse[of "mp\<^sub>2 (pid,vs)", simplified, OF q_pos]
+      using fraction_consistent_external(1)[OF WfCtxt extcons\<^sub>a, of "mp\<^sub>2 (pid, vs) / mp (pid, vs)", unfolded \<open>Rep_posreal q\<^sub>a = _\<close>, simplified]
+      by (metis (mono_tags, lifting) Rep_preal_inject \<open>mp\<^sub>2 (pid, vs) \<le> mp (pid, vs)\<close> divide_preal.rep_eq dual_order.strict_trans1 nonzero_eq_divide_eq pperm_pgt_pnone q_pos times_preal.rep_eq zero_preal.rep_eq)
+  qed
+
+  have "nm\<^sub>1 + nm\<^sub>2 = nm"
+    unfolding plus_nested_mask_def nm\<^sub>1 nm\<^sub>2
+    apply simp
+    apply (rule nested_mask_equality)
+    using IH.hyps(1) IH.prems(1)
+     apply auto[1]
+    unfolding fnm[symmetric]
+    apply simp
+    apply standard
+    apply (rename_tac lp)
+    apply (case_tac "fnm\<^sub>1 lp"; case_tac "fnm\<^sub>2 lp"; simp add: pfun_comb_def)
+    subgoal for lp
+      apply (subgoal_tac "mp lp = 0")
+       apply (metis IH.prems(2) fnm get_mp_0_implies_fnm_None)
+      apply (subgoal_tac "mp\<^sub>1 lp = 0 \<and> mp\<^sub>2 lp = 0")
+      using IH(2)[simplified, THEN fun_cong, of lp, simplified add_masks_def]
+       apply fastforce
+      using fnm\<^sub>1[of lp] fnm\<^sub>2[of lp]
+      by (metis option.distinct(1))
+    subgoal for lp lpm\<^sub>2
+      apply (subgoal_tac "mp\<^sub>1 lp = 0 \<and> mp\<^sub>2 lp = mp lp \<and> mp\<^sub>2 lp > 0")
+      using fnm\<^sub>2[of lp, simplified]
+       apply (metis IH.prems(2) PosReal.field_divide_inverse PosReal.field_inverse Some_Some_ifD fnm obtain_lpm_from_mp option.sel pos_perm_class.pmult_comm preal_semimodule_class.scale_one snd_conv)
+      using IH(2)[simplified, THEN fun_cong, of lp, simplified add_masks_def]
+      by (metis add.commute fnm\<^sub>1 fnm\<^sub>2 option.distinct(1) padd_pnone preal_not_0_gt_0)
+    subgoal for lp lpm\<^sub>1
+      apply (subgoal_tac "mp\<^sub>2 lp = 0 \<and> mp\<^sub>1 lp = mp lp \<and> mp\<^sub>1 lp > 0")
+      using fnm\<^sub>2[of lp, simplified]
+       apply (metis IH.prems(2) PosReal.field_divide_inverse PosReal.field_inverse fnm fnm\<^sub>1 obtain_lpm_from_mp option.sel order_less_le pos_perm_class.pmult_comm preal_semimodule_class.scale_one snd_conv)
+      using IH(2)[simplified, THEN fun_cong, of lp, simplified add_masks_def]
+      by (metis fnm\<^sub>1 fnm\<^sub>2 option.distinct(1) padd_pnone preal_not_0_gt_0)
+    subgoal for lp lpm\<^sub>1 lpm\<^sub>2
+    proof -
+      assume "fnm\<^sub>1 lp = Some lpm\<^sub>1"
+        and "fnm\<^sub>2 lp = Some lpm\<^sub>2"
+      have "Rep_posreal (fst lpm\<^sub>1) = mp\<^sub>1 lp"
+        using \<open>fnm\<^sub>1 lp = Some lpm\<^sub>1\<close> \<open>mp\<^sub>1 = get_mp_nm nm\<^sub>1\<close> nm\<^sub>1 by auto
+      have "Rep_posreal (fst lpm\<^sub>2) = mp\<^sub>2 lp"
+        using \<open>fnm\<^sub>2 lp = Some lpm\<^sub>2\<close> \<open>mp\<^sub>2 = get_mp_nm nm\<^sub>2\<close> nm\<^sub>2 by auto
+      have "mp lp > 0"
+        by (metis IH.hyps(2) \<open>fnm\<^sub>1 lp = Some lpm\<^sub>1\<close> fnm\<^sub>1 le_funD option.distinct(1) order_less_imp_not_less order_less_le preal_not_0_gt_0 split_implies_le(1))
+      hence 1: "fnm lp = Some (Abs_posreal (mp lp), snd (the (fnm lp)))"
+        by (metis IH.prems(2) fnm obtain_lpm_from_mp option.sel split_pairs)
+      have 2: "snd lpm\<^sub>1 = (mp\<^sub>1 lp / mp lp) *\<^sub>s snd (the (fnm lp))"
+        by (metis \<open>fnm\<^sub>1 lp = Some lpm\<^sub>1\<close> fnm\<^sub>1 option.discI option.sel split_pairs)
+      have 3: "snd lpm\<^sub>2 = (mp\<^sub>2 lp / mp lp) *\<^sub>s snd (the (fnm lp))"
+        by (metis \<open>fnm\<^sub>2 lp = Some lpm\<^sub>2\<close> fnm\<^sub>2 option.discI option.sel split_pairs)
+      show "Some (fst lpm\<^sub>1 + fst lpm\<^sub>2, nested_mask_merge (snd lpm\<^sub>1) (snd lpm\<^sub>2)) = fnm lp"
+        apply (subst 1)
+        apply standard+
+         apply (rule Rep_posreal_inject[THEN iffD1])
+        unfolding plus_posreal.rep_eq
+         apply (metis Abs_posreal_inject IH.hyps(2) Rep_posreal Rep_posreal_inverse \<open>Rep_posreal (fst lpm\<^sub>1) = mp\<^sub>1 lp\<close> \<open>Rep_posreal (fst lpm\<^sub>2) = mp\<^sub>2 lp\<close> \<open>pos_perm_class.pnone < mp lp\<close> add_masks_def mem_Collect_eq mp_split.simps)
+        unfolding plus_nested_mask_def[symmetric] 2 3
+        unfolding preal_semimodule_class.scale_add_left[symmetric]
+        using preal_semimodule_class.scale_one IH(2)[simplified, THEN fun_cong, of lp, simplified add_masks_def]
+        by (metis PosReal.field_divide_inverse PosReal.field_inverse PosReal.pmult_comm \<open>pos_perm_class.pnone < mp lp\<close> distrib_right preal_not_0_gt_0)
+    qed
+    done
+
+  define \<omega>\<^sub>A where "\<omega>\<^sub>A = add_to_nm_total_full \<omega> nm\<^sub>1"
+  have 1: "add_to_nm_total_full \<omega>\<^sub>A nm\<^sub>2 = add_to_nm_total_full \<omega> nm"
+    apply (rule full_total_state.equality; simp_all add: IH \<omega>\<^sub>A_def)
+    apply (rule total_state.equality; simp_all add: IH \<omega>\<^sub>A_def)
+    using \<open>nm\<^sub>1 + nm\<^sub>2 = nm\<close> ab_semigroup_add_class.add_ac(1)
+    by blast
+
+  have "add_to_nm_total_full \<omega> nm \<succeq> add_to_nm_total_full \<omega> nm\<^sub>1"
+    apply (simp add: greater_def)
+    apply (rule exI[of _ "upd_nm_total_full \<omega> nm\<^sub>2"])
+    apply (simp add: plus_full_total_state_ext_def)
+    apply standard+
+     apply (metis (no_types, lifting) \<open>nm\<^sub>1 + nm\<^sub>2 = nm\<close> ab_semigroup_add_class.add_ac(1) option.sel plus_total_state_ext_def total_state.ext_inject total_state.surjective total_state.update_convs(2))
+    by (simp add: defined_def plus_total_state_ext_def)
+  hence A_mask_intcons: "StateCons (add_to_nm_total_full \<omega> nm\<^sub>1)"
+    using IH(14) MonoCons mono_prop_downwardD
+    by blast
+
+  show ?case
+    apply (rule InhStarNormal[where ?\<omega>''=\<omega>\<^sub>A])
+    unfolding \<open>\<omega>\<^sub>A = _\<close>
+    using IH(5)[of nm\<^sub>1 \<omega>]
+    apply (metis A_mask_intcons A_sup IH.prems(4) IH.prems(5) IH.prems(6) \<open>mp\<^sub>1 = _\<close> assertion_framing_star get_mh_nm.simps nm\<^sub>1 nm\<^sub>1_cons)
+    using IH(6)[of nm\<^sub>2 \<omega>\<^sub>A, OF _ _ nm\<^sub>2_cons] 1
+    by (metis A_mask_intcons A_sup B_sup IH.IH(1) IH.prems(4) IH.prems(5) IH.prems(6) IH.prems(8) \<omega>\<^sub>A_def \<open>mp\<^sub>1 = _\<close> \<open>mp\<^sub>2 = _\<close> assertion_framing_star get_mh_nm.simps inhale_only_changes_mask nm\<^sub>1 nm\<^sub>1_cons nm\<^sub>2)
+
+next
+  case IH: (SatImpTrue e mh mp A)
+
+  hence e_sup: "supported_pred_expr e" and A_sup: "supported_pred_body A"
+    by simp+
+  obtain res where res: "ctxt, Some \<omega> \<turnstile> \<langle>e;\<omega>\<rangle> [\<Down>]\<^sub>t res"
+    by (metis IH.hyps(1) IH.prems(4) IH.prems(5) \<omega>\<^sub>0hh e_sup eval_ok_no_type_error(1))
+
+  show ?case
+  proof (cases res)
+    case (Val v\<^sub>2)
+    hence "v\<^sub>2 = VBool True"
+      using eval_with_same_store_same_hh(1)[OF IH(1) res _ Val e_sup] IH.prems(4) IH.prems(5) \<omega>\<^sub>0hh
+      by presburger
+    show ?thesis
+      apply (rule InhImpTrue)
+      using Val \<open>v\<^sub>2 = VBool True\<close> res
+       apply blast
+      using IH(3)[OF IH(4-8)] A_sup Val \<open>v\<^sub>2 = VBool True\<close> assertion_framing_imp res IH.prems(6,8)
+      by blast
+  next
+    case VFailure
+    then show ?thesis
+      using IH.prems(6) res assertion_framing_state_def inh_imp_failure by blast
+  qed
+
+next
+  case IH: (SatImpFalse e mh mp A)
+
+  hence e_sup: "supported_pred_expr e" and A_sup: "supported_pred_body A"
+    by simp+
+  obtain res where res: "ctxt, Some \<omega> \<turnstile> \<langle>e;\<omega>\<rangle> [\<Down>]\<^sub>t res"
+    by (metis IH.hyps(1) IH.prems(4) IH.prems(5) \<omega>\<^sub>0hh e_sup eval_ok_no_type_error(1))
+
+  have "nm = 0"
+    apply (simp add: zero_nested_mask_def)
+    apply (rule nested_mask_equality, simp_all)
+    using IH.hyps(2) IH.prems(1) zero_mask_def
+      apply fastforce
+    using IH.hyps(3) IH.prems(2) zero_mask_def
+    by (metis get_mp_0_implies_fnm_None)
+
+  show ?case
+  proof (cases res)
+    case (Val v\<^sub>2)
+    hence "v\<^sub>2 = VBool False"
+      using eval_with_same_store_same_hh(1)[OF IH(1) res _ Val e_sup] IH.prems(4) IH.prems(5) \<omega>\<^sub>0hh
+      by presburger
+    show ?thesis
+      apply (rule InhImpFalse)
+      using Val \<open>v\<^sub>2 = VBool False\<close> res
+       apply blast
+      by (simp add: \<open>nm = 0\<close>)
+  next
+    case VFailure
+    then show ?thesis
+      using IH.prems(6) res assertion_framing_state_def inh_imp_failure by blast
+  qed
+
+next
+  case IH: (SatCondTrue e mh mp A B)
+
+  hence e_sup: "supported_pred_expr e" and A_sup: "supported_pred_body A" and B_sup: "supported_pred_body B"
+    by simp+
+  obtain res where res: "ctxt, Some \<omega> \<turnstile> \<langle>e;\<omega>\<rangle> [\<Down>]\<^sub>t res"
+    by (metis IH.hyps(1) IH.prems(4) IH.prems(5) \<omega>\<^sub>0hh e_sup eval_ok_no_type_error(1))
+
+  show ?case
+  proof (cases res)
+    case (Val v\<^sub>2)
+    hence "v\<^sub>2 = VBool True"
+      using eval_with_same_store_same_hh(1)[OF IH(1) res _ Val e_sup] IH.prems(4) IH.prems(5) \<omega>\<^sub>0hh
+      by presburger
+    show ?thesis
+      apply (rule InhCondAssertTrue)
+      using Val \<open>v\<^sub>2 = VBool True\<close> res
+       apply blast
+      using IH(3)[OF IH(4-8)] A_sup Val \<open>v\<^sub>2 = VBool True\<close> assertion_framing_cond_assert_true res IH.prems(6,8)
+      by blast
+  next
+    case VFailure
+    then show ?thesis
+      using IH.prems(6) res assertion_framing_state_def inh_cond_assert_failure by blast
+  qed
+
+next
+  case IH: (SatCondFalse e mh mp B A)
+
+  hence e_sup: "supported_pred_expr e" and A_sup: "supported_pred_body A" and B_sup: "supported_pred_body B"
+    by simp+
+  obtain res where res: "ctxt, Some \<omega> \<turnstile> \<langle>e;\<omega>\<rangle> [\<Down>]\<^sub>t res"
+    by (metis IH.hyps(1) IH.prems(4) IH.prems(5) \<omega>\<^sub>0hh e_sup eval_ok_no_type_error(1))
+
+  show ?case
+  proof (cases res)
+    case (Val v\<^sub>2)
+    hence "v\<^sub>2 = VBool False"
+      using eval_with_same_store_same_hh(1)[OF IH(1) res _ Val e_sup] IH.prems(4) IH.prems(5) \<omega>\<^sub>0hh
+      by presburger
+    show ?thesis
+      apply (rule InhCondAssertFalse)
+      using Val \<open>v\<^sub>2 = VBool False\<close> res
+       apply blast
+      by (metis B_sup IH.IH IH.prems(1-6,8) Val \<open>v\<^sub>2 = VBool False\<close> assertion_framing_cond_assert_false res)
+  next
+    case VFailure
+    then show ?thesis
+      using IH.prems(6) res assertion_framing_state_def inh_cond_assert_failure by blast
+  qed
+qed
+
+
+lemma extcons_state_can_be_inhaled:
+  assumes PredDecl: "ViperLang.predicates (program_total ctxt) pid = Some pdecl"
+      and PredBody: "ViperLang.predicate_decl.body pdecl = Some pbody"
+      and SupPred: "supported_pred_body pbody"
+      and SelfFraming: "\<And>q. assertion_framing_state ctxt StateCons (syntactic_mult q pbody) \<omega>"
+      and ExtCons: "consistent_external_wrt_ploc ctxt \<lparr> get_hh_total = hh, get_nm_total = nm \<rparr> (pid,vs) p"
+      and \<omega>hh: "get_hh_total_full \<omega> = hh"
+      and \<omega>Store: "get_store_total \<omega> = nth_option vs"
+      and FinalIntCons: "StateCons (add_to_nm_total_full \<omega> nm)"
+      and MonoCons: "mono_prop_downward StateCons"
+      and WfCtxt: "ctxt_pred_syn_wf ctxt"
+      and "p > 0"
+    shows "red_inhale ctxt StateCons (syntactic_mult (Rep_preal p) pbody) \<omega> (RNormal (add_to_nm_total_full \<omega> nm))"
+proof -
+  have
+    "vals_well_typed (absval_interp_total ctxt) vs (predicate_decl.args pdecl)"
+    "p = 0 \<Longrightarrow> nm = 0" and
+    "p > 0 \<Longrightarrow> sat ctxt \<lparr> get_store_total = nth_option vs,
+                   get_trace_total = Map.empty,
+                   get_total_full = \<lparr> get_hh_total = hh, get_nm_total = 0 \<rparr> \<rparr>
+            (get_mh_nm nm) (get_mp_nm nm)
+            (syntactic_mult (Rep_preal p) pbody)" and
+    "consistent_external ctxt \<lparr> get_hh_total = hh, get_nm_total = nm \<rparr>"
+    using SatStep_case PredDecl PredBody ExtCons
+    by fastforce+
+  moreover have "assertion_framing_state ctxt StateCons (syntactic_mult (Rep_preal p) pbody) \<omega>"
+    using SelfFraming
+    by (simp add: calculation(1))
+  ultimately show ?thesis
+    apply (cases "p > 0")
+    using \<omega>Store \<omega>hh extcons_state_can_be_inhaled_assertion FinalIntCons MonoCons
+     apply (metis SupPred WfCtxt full_total_state.select_convs(1) full_total_state.select_convs(3) get_hh_total_full.simps prat_non_negative syntactic_mult_supported total_state.select_convs(1))
+    apply (subgoal_tac "p = 0")
+     prefer 2
+    using preal_not_0_gt_0
+     apply blast
+    apply simp
+    using assms(11)
+    by blast
+qed
+
+
+
 subsection \<open>Inhale Properties\<close>
 
 lemma inhale_with_more_variables:
@@ -983,16 +1757,1143 @@ lemma inhale_mono:
 
 
 
-subsection \<open>Framed Evaluation Properties\<close>
+subsection \<open>Relation between Two Self-Framing Definitions\<close>
 
 
-lemma eval_hh_decides_well_typedness:
-  assumes "get_hh_total_full \<omega>\<^sub>1 = get_hh_total_full \<omega>\<^sub>2"
-    shows "ctxt, \<omega>_def\<^sub>1 \<turnstile> \<langle>e;\<omega>\<^sub>1\<rangle> [\<Down>]\<^sub>t r\<^sub>1 \<Longrightarrow>
-           \<exists>r\<^sub>2. ctxt, \<omega>_def\<^sub>2 \<turnstile> \<langle>e;\<omega>\<^sub>2\<rangle> [\<Down>]\<^sub>t r\<^sub>2"
-      and "red_pure_exps_total ctxt \<omega>_def\<^sub>1 es \<omega>\<^sub>1 rs\<^sub>1 \<Longrightarrow>
-           \<exists>rs\<^sub>2. red_pure_exps_total ctxt \<omega>_def\<^sub>2 es \<omega>\<^sub>2 rs\<^sub>2"
+lemma eval_perm_0_locs_irrelevant:
+  assumes "get_store_total \<omega>\<^sub>0 = get_store_total \<omega>\<^sub>0'"
+      and "get_trace_total \<omega>\<^sub>0 = get_trace_total \<omega>\<^sub>0'"
+      and "differ_only_in_0_perm_locs (get_total_full \<omega>\<^sub>0) (get_total_full \<omega>\<^sub>0')"
+      and "get_store_total \<omega> = get_store_total \<omega>'"
+      and "get_trace_total \<omega> = get_trace_total \<omega>'"
+      and "get_nm_total_full \<omega> = get_nm_total_full \<omega>'"
+      and "get_hh_total_full \<omega>\<^sub>0 = get_hh_total_full \<omega>"
+      and "get_hh_total_full \<omega>\<^sub>0' = get_hh_total_full \<omega>'"
+      and "\<omega>_def = Some \<omega>\<^sub>0"
+      and "\<omega>_def' = Some \<omega>\<^sub>0'"
+    shows "ctxt, \<omega>_def \<turnstile> \<langle>e;\<omega>\<rangle> [\<Down>]\<^sub>t r \<Longrightarrow>
+           r \<noteq> VFailure \<Longrightarrow>
+           ctxt, \<omega>_def' \<turnstile> \<langle>e;\<omega>'\<rangle> [\<Down>]\<^sub>t r"
+      and "red_pure_exps_total ctxt \<omega>_def es \<omega> rs \<Longrightarrow>
+           rs \<noteq> None \<Longrightarrow>
+           red_pure_exps_total ctxt \<omega>_def' es \<omega>' rs"
+  using assms
+proof (induction arbitrary: \<omega>\<^sub>0 \<omega>_def' \<omega>\<^sub>0' \<omega>' and \<omega>\<^sub>0 \<omega>_def' \<omega>\<^sub>0' \<omega>' rule: red_pure_exp_inducts)
+  case IH: (RedBinopLazy \<omega>_def e1 \<omega> v1 bop v e2)
+  then show ?case
+    by (fastforce intro: RedBinopLazy)
+next
+  case IH: (RedBinop \<omega>_def e1 \<omega> v1 e2 v2 bop v)
+  then show ?case
+    by (fastforce intro: RedBinop)
+next
+  case IH: (RedUnop \<omega>_def e \<omega> v unop v')
+  then show ?case
+    by (fastforce intro: RedUnop)
+next
+  case IH: (RedOld \<omega> l \<phi> \<omega>_def'\<^sub>s \<omega>_def e v)
+  show ?case
+    apply (rule TotalExpressions.RedOld)
+    using IH
+      apply simp
+    using IH
+     apply simp
+    using IH(3)[unfolded \<open>\<omega>_def'\<^sub>s = _\<close> \<open>\<omega>_def = _\<close>, simplified]
+    apply (subgoal_tac "\<omega>\<^sub>0\<lparr> get_total_full := \<phi> \<rparr> = \<omega>\<^sub>0'\<lparr> get_total_full := \<phi> \<rparr>")
+     apply (subgoal_tac "\<omega>\<lparr> get_total_full := \<phi> \<rparr> = \<omega>'\<lparr> get_total_full := \<phi> \<rparr>")
+      apply argo
+    by (rule full_total_state.equality, simp_all add: IH)
+next
+  case IH: (RedField \<omega>_def e \<omega> a f v)
+  have **: "ctxt, \<omega>_def' \<turnstile> \<langle>e;\<omega>'\<rangle> [\<Down>]\<^sub>t Val (VRef (Address a))"
+    by (metis IH.IH(2) IH.prems(2-11) extended_val.distinct(1))
+  show ?case
+    unfolding \<open>\<omega>_def = _\<close> \<open>\<omega>_def' = _\<close>
+    apply simp
+    apply (intro conjI)
+     defer
+    using IH.prems(1,10)
+     apply force
+  proof
+    assume "(a,f) \<in> get_valid_locs \<omega>\<^sub>0"
+    hence "(a,f) \<in> get_valid_locs \<omega>\<^sub>0'"
+      using IH(7)[unfolded differ_only_in_0_perm_locs_def]
+      unfolding get_valid_locs_def
+      by auto
+    moreover have "get_hh_total_full \<omega>' (a,f) = v"
+      unfolding IH(12)[symmetric]
+      using IH(7)[unfolded differ_only_in_0_perm_locs_def]
+      by (metis IH.hyps IH.prems(8) \<open>(a, f) \<in> get_valid_locs \<omega>\<^sub>0\<close> get_hh_total_full.simps get_mh_total.simps get_mh_total_full.simps get_valid_locs_def mem_Collect_eq pperm_pgt_pnone sum_0_implies_mh_zero)
+    ultimately show "ctxt, Some \<omega>\<^sub>0' \<turnstile> \<langle>FieldAcc e f;\<omega>'\<rangle> [\<Down>]\<^sub>t Val v"
+      using ** IH.prems(11) RedField_def_normalI
+      by blast
+  qed
+next
+  case IH: (RedPerm \<omega>_def e \<omega> a f v)
+  then show ?case
+    by (fastforce intro: RedPerm)
+next
+  case IH: (RedUnfoldingDef \<omega>\<^sub>0\<^sub>f es \<omega> vs perm pid nm' \<omega>\<^sub>0\<^sub>u ubody v)
+  hence *: "get_nm_total_full \<omega>\<^sub>0 = get_nm_total_full \<omega>\<^sub>0'"
+    by (metis differ_only_in_0_perm_locs_def get_nm_total_full.simps)
+  have "\<omega>\<^sub>0\<^sub>f = \<omega>\<^sub>0"
+    using IH.prems(10)
+    by auto
+  define perm' where "perm' = get_mp_total_full \<omega>\<^sub>0' (pid,vs)"
+  have **: "\<And>l. nm_loc_sum l (get_nm_total_full \<omega>\<^sub>0) 0 \<Longrightarrow> nm_loc_sum l nm' 0"
+    using IH.hyps(3) \<open>\<omega>\<^sub>0\<^sub>f = \<omega>\<^sub>0\<close> shift_up_preserves_loc_sum
+    by blast
+
+  show ?case
+    unfolding \<open>\<omega>_def' = _\<close>
+    apply (rule RedUnfoldingDef)
+         apply (rule IH(2)[of \<omega>\<^sub>0 \<omega>\<^sub>0'])
+                   apply simp
+                  apply fact+
+         apply simp
+        apply fact
+    unfolding \<open>perm' = _\<close>
+    using IH.hyps(1,2) * \<open>\<omega>\<^sub>0\<^sub>f = \<omega>\<^sub>0\<close>
+       apply auto[1]
+    using IH *
+      apply simp
+     apply (simp del: upd_nm_total_full.simps)
+    apply (rule IH(4)[of \<omega>\<^sub>0\<^sub>u "upd_nm_total_full \<omega>\<^sub>0' nm'"])
+              apply auto
+            apply (simp add: IH.prems(1))
+           apply (simp add: IH.hyps(4) IH.prems(2) \<open>\<omega>\<^sub>0\<^sub>f = \<omega>\<^sub>0\<close>)
+          apply (simp add: IH.hyps(4) IH.prems(3) \<open>\<omega>\<^sub>0\<^sub>f = \<omega>\<^sub>0\<close>)
+    using IH(12)
+    unfolding differ_only_in_0_perm_locs_def
+    using ** IH.hyps(4) \<open>\<omega>\<^sub>0\<^sub>f = \<omega>\<^sub>0\<close>
+         apply force
+        apply fact+
+    using IH.hyps(4) IH.prems(7-9) \<open>\<omega>\<^sub>0\<^sub>f = \<omega>\<^sub>0\<close>
+    by auto
+next
+  case (RedExpListCons \<omega>_def e \<omega> v es res res')
+  then show ?case
+    by (metis extended_val.distinct(1) option.simps(8) red_pure_exp_total_red_pure_exps_total.RedExpListCons)
+qed (auto intro: red_pure_exp_intros)
+
+
+lemma eval_perm_0_locs_irrelevant_supported_pred:
+  assumes "get_store_total \<omega>\<^sub>0 = get_store_total \<omega>\<^sub>0'"
+      and "differ_only_in_0_perm_locs (get_total_full \<omega>\<^sub>0) (get_total_full \<omega>\<^sub>0')"
+      and "get_store_total \<omega> = get_store_total \<omega>'"
+      and "get_hh_total_full \<omega>\<^sub>0 = get_hh_total_full \<omega>"
+      and "get_hh_total_full \<omega>\<^sub>0' = get_hh_total_full \<omega>'"
+      and "\<omega>_def = Some \<omega>\<^sub>0"
+      and "\<omega>_def' = Some \<omega>\<^sub>0'"
+    shows "ctxt, \<omega>_def \<turnstile> \<langle>e;\<omega>\<rangle> [\<Down>]\<^sub>t r \<Longrightarrow>
+           r \<noteq> VFailure \<Longrightarrow>
+           supported_pred_expr e \<Longrightarrow>
+           ctxt, \<omega>_def' \<turnstile> \<langle>e;\<omega>'\<rangle> [\<Down>]\<^sub>t r"
+      and "red_pure_exps_total ctxt \<omega>_def es \<omega> rs \<Longrightarrow>
+           rs \<noteq> None \<Longrightarrow>
+           list_all supported_pred_expr es \<Longrightarrow>
+           red_pure_exps_total ctxt \<omega>_def' es \<omega>' rs"
+  using assms
+proof (induction arbitrary: \<omega>\<^sub>0 \<omega>_def' \<omega>\<^sub>0' \<omega>' and \<omega>\<^sub>0 \<omega>_def' \<omega>\<^sub>0' \<omega>' rule: red_pure_exp_inducts)
+  case IH: (RedBinopLazy \<omega>_def e1 \<omega> v1 bop v e2)
+  then show ?case
+    by (fastforce intro: RedBinopLazy)
+next
+  case IH: (RedBinop \<omega>_def e1 \<omega> v1 e2 v2 bop v)
+  then show ?case
+    by (fastforce intro: RedBinop)
+next
+  case IH: (RedUnop \<omega>_def e \<omega> v unop v')
+  then show ?case
+    by (fastforce intro: RedUnop)
+next
+  case IH: (RedField \<omega>_def e \<omega> a f v)
+  have **: "ctxt, \<omega>_def' \<turnstile> \<langle>e;\<omega>'\<rangle> [\<Down>]\<^sub>t Val (VRef (Address a))"
+    using IH.IH(2) IH.prems(2-9)
+    by auto
+  show ?case
+    unfolding \<open>\<omega>_def = _\<close> \<open>\<omega>_def' = _\<close>
+    apply simp
+    apply (intro conjI)
+     defer
+    using IH.prems(1,8)
+     apply force
+  proof
+    assume "(a,f) \<in> get_valid_locs \<omega>\<^sub>0"
+    hence "(a,f) \<in> get_valid_locs \<omega>\<^sub>0'"
+      using IH(7)[unfolded differ_only_in_0_perm_locs_def]
+      unfolding get_valid_locs_def
+      by auto
+    moreover have "get_hh_total_full \<omega>' (a,f) = v"
+      unfolding IH(12)[symmetric]
+      using IH(7)[unfolded differ_only_in_0_perm_locs_def]
+      by (metis IH.hyps IH.prems(6,7) \<open>(a, f) \<in> get_valid_locs \<omega>\<^sub>0\<close> get_hh_total_full.simps get_mh_total.simps get_mh_total_full.simps get_valid_locs_def mem_Collect_eq pperm_pgt_pnone sum_0_implies_mh_zero)
+    ultimately show "ctxt, Some \<omega>\<^sub>0' \<turnstile> \<langle>FieldAcc e f;\<omega>'\<rangle> [\<Down>]\<^sub>t Val v"
+      using ** IH.prems(9) RedField_def_normalI
+      by blast
+  qed
+next
+  case IH: (RedUnfoldingDef \<omega>\<^sub>0\<^sub>f es \<omega> vs perm pid nm' \<omega>\<^sub>0\<^sub>u ubody v)
+  hence *: "get_nm_total_full \<omega>\<^sub>0 = get_nm_total_full \<omega>\<^sub>0'"
+    by (metis differ_only_in_0_perm_locs_def get_nm_total_full.simps)
+  have "\<omega>\<^sub>0\<^sub>f = \<omega>\<^sub>0"
+    using IH.prems(8)
+    by auto
+  define perm' where "perm' = get_mp_total_full \<omega>\<^sub>0' (pid,vs)"
+  have **: "\<And>l. nm_loc_sum l (get_nm_total_full \<omega>\<^sub>0) 0 \<Longrightarrow> nm_loc_sum l nm' 0"
+    using IH.hyps(3) \<open>\<omega>\<^sub>0\<^sub>f = \<omega>\<^sub>0\<close> shift_up_preserves_loc_sum
+    by blast
+
+  show ?case
+    unfolding \<open>\<omega>_def' = _\<close>
+    apply (rule RedUnfoldingDef)
+         apply (rule IH(2)[of \<omega>\<^sub>0 \<omega>\<^sub>0'])
+                 apply simp
+    using IH.prems(2) supported_sub_expr_supported
+                apply fastforce
+               apply fact+
+         apply simp
+        apply fact
+    unfolding \<open>perm' = _\<close>
+    using IH.hyps(1,2) * \<open>\<omega>\<^sub>0\<^sub>f = \<omega>\<^sub>0\<close>
+       apply auto[1]
+    using IH *
+      apply simp
+     apply (simp del: upd_nm_total_full.simps)
+    apply (rule IH(4)[of \<omega>\<^sub>0\<^sub>u "upd_nm_total_full \<omega>\<^sub>0' nm'"])
+            apply (simp add: IH.prems(1))
+    using IH.prems(2)
+           apply auto[1]
+          apply (simp add: IH.hyps(4) IH.prems(3) \<open>\<omega>\<^sub>0\<^sub>f = \<omega>\<^sub>0\<close>)
+    using IH(12)
+    unfolding differ_only_in_0_perm_locs_def
+    using ** IH.hyps(4) \<open>\<omega>\<^sub>0\<^sub>f = \<omega>\<^sub>0\<close>
+         apply force
+        apply fact
+    using IH.hyps(4) IH.prems(6) \<open>\<omega>\<^sub>0\<^sub>f = \<omega>\<^sub>0\<close>
+       apply auto[1]
+    using IH.hyps(4) IH.prems(7-9) \<open>\<omega>\<^sub>0\<^sub>f = \<omega>\<^sub>0\<close>
+    by auto
+next
+  case (RedExpListCons \<omega>_def e \<omega> v es res res')
+  then show ?case
+    by (fastforce intro: red_pure_exp_total_red_pure_exps_total.RedExpListCons)
+qed (auto intro: red_pure_exp_intros)
+
+
+lemma eval_None_same_hh:  \<comment> \<open>redundant with @{thm eval_exhale_sat_helper_helper}}\<close>
+  assumes "get_hh_total_full \<omega> = get_hh_total_full \<omega>'"
+      and "get_store_total \<omega> = get_store_total \<omega>'"
+    shows "ctxt, \<omega>_def \<turnstile> \<langle>e;\<omega>\<rangle> [\<Down>]\<^sub>t r \<Longrightarrow>
+           \<omega>_def = None \<Longrightarrow>
+           r = Val v \<Longrightarrow>
+           supported_pred_expr e \<Longrightarrow>
+           ctxt, None \<turnstile> \<langle>e;\<omega>'\<rangle> [\<Down>]\<^sub>t Val v"
+      and "red_pure_exps_total ctxt \<omega>_def es \<omega> rs \<Longrightarrow>
+           \<omega>_def = None \<Longrightarrow>
+           rs = Some vs \<Longrightarrow>
+           list_all supported_pred_expr es \<Longrightarrow>
+           red_pure_exps_total ctxt None es \<omega>' (Some vs)"
+  using assms
+proof (induction arbitrary: \<omega>' v and \<omega>' vs rule: red_pure_exp_inducts)
+  case (RedField \<omega>_def e \<omega> a f v)
+  then show ?case
+    by (metis RedField_no_def_normalI eval_exhale_sat_helper_helper(1) option.pred_inject(1))
+next
+  case (RedUnfolding es \<omega> vs ubody v pred_id)
+  then show ?case
+    by (meson eval_exhale_sat_helper_helper(1) red_pure_exp_total_red_pure_exps_total.RedUnfolding)
+qed (fastforce intro: red_pure_exp_intros)+
+
+
+lemma framed_sat_irrelevant_perm_0_locs_helper:
+    fixes \<phi> :: "'a total_state"
+  assumes "red_pure_exps_total ctxt None es \<omega> (Some vs)"
+      and Framed: "assertion_framing_state ctxt StateCons A \<omega>\<^sub>0"
+      and hh_diff_only: "differ_only_in_0_perm_locs_hh (add_to_nm_total \<phi> (get_nm_total_full \<omega>\<^sub>0)) hh"
+      and "get_store_total \<omega>\<^sub>0 = get_store_total \<omega>"
+      and "get_hh_total_full \<omega>\<^sub>0 = get_hh_total_full \<omega>"
+      and "get_hh_total_full \<omega> = get_hh_total \<phi>"
+      and "get_hh_total_full \<omega>' = hh"
+      and "get_store_total \<omega>\<^sub>0 = get_store_total \<omega>'"
+      and "supported_pred_body A"
+      and "es = direct_sub_expressions_assertion A"
+    shows "red_pure_exps_total ctxt None es \<omega>' (Some vs)" (is ?P1)
+      and "red_pure_exps_total ctxt (Some \<omega>\<^sub>0) es \<omega>\<^sub>0 (Some vs)" (is ?P2)
+proof -
+  \<comment> \<open>Evaluating \<^term>\<open>es\<close> under \<^term>\<open>\<omega>\<^sub>0\<close> does not result in a type error.\<close>
+  have "\<exists>rs. red_pure_exps_total ctxt (Some \<omega>\<^sub>0) es \<omega>\<^sub>0 rs"
+    apply (rule eval_ok_no_type_error(2)[OF _ _ assms(1)])
+    using assms(4,5)
+       apply (force, force)
+     apply simp
+    by (metis (no_types, lifting) assert_pred_subexp assms(9,10) list_all_length)
+
+  \<comment> \<open>Since, the assertion \<^term>\<open>A\<close> is framed by \<^term>\<open>\<omega>\<^sub>0\<close>, the evaluation of direct sub-expressions cannot fail.\<close>
+  then obtain vs' where "red_pure_exps_total ctxt (Some \<omega>\<^sub>0) es \<omega>\<^sub>0 (Some vs')"
+    using Framed[unfolded assertion_framing_state_def] InhSubExpFailure \<open>es = _\<close>
+    by (metis red_exp_list_failure_Nil split_option_ex)
+
+  \<comment> \<open>The evaluation result is the same.\<close>
+  thus ?P2
+    by (metis assert_pred_subexp assms(1,4,5,9,10) eval_exhale_sat_helper_helper(2) eval_is_deterministic(2))
+
+  \<comment> \<open>Change the underlying state to \<^term>\<open>\<omega>'\<close>.\<close>
+  have "red_pure_exps_total ctxt (Some (upd_hh_total_full \<omega>\<^sub>0 (get_hh_total_full \<omega>'))) es \<omega>' (Some vs)"
+    apply (rule eval_perm_0_locs_irrelevant_supported_pred(2)[where \<omega>\<^sub>0=\<omega>\<^sub>0 and \<omega>=\<omega>\<^sub>0 and \<omega>\<^sub>0'="upd_hh_total_full \<omega>\<^sub>0 (get_hh_total_full \<omega>')"]; (rule assms)?)  \<comment> \<open>The instantiation of \<^term>\<open>\<omega>\<^sub>0'\<close> is weird. But it does the trick. Could generalize @{thm eval_perm_0_locs_irrelevant_supported_pred} to unrestrict \<^term>\<open>hh\<close> of well-definedness states.\<close>
+            apply simp
+    unfolding differ_only_in_0_perm_locs_def
+           apply (intro conjI)
+            apply simp
+    using hh_diff_only[unfolded differ_only_in_0_perm_locs_hh_def]
+            apply (metis add.commute add_to_nm_total.simps all_pos assms(5) assms(6) assms(7) get_hh_total_full.simps get_nm_total_full.simps nle_le nm_loc_sum.elims(2) nm_loc_sum_smaller nm_sum_is_bigger total_state.select_convs(1) total_state.select_convs(2) total_state.surjective total_state.update_convs(2))
+           prefer 8
+           apply (metis (no_types, lifting) assert_pred_subexp assms(10) assms(9) list_all_length)
+          apply simp_all
+    by fact
+
+  thus ?P1
+    by (metis assert_pred_subexp assms(9,10) eval_exhale_sat_helper_helper(2))
+qed
+
+
+lemma eval_list_2D:
+  assumes "red_pure_exps_total ctxt \<omega>_def [e1, e2] \<omega> (Some [v1, v2])"
+    shows "ctxt, \<omega>_def \<turnstile> \<langle>e1;\<omega>\<rangle> [\<Down>]\<^sub>t Val v1"
+      and "ctxt, \<omega>_def \<turnstile> \<langle>e2;\<omega>\<rangle> [\<Down>]\<^sub>t Val v2"
+  using assms
+  by (fastforce elim: red_exp_list_normal_elim)+
+
+
+lemma eval_list_append_to_oneD:
+  assumes "red_pure_exps_total ctxt \<omega>_def (es @ [e]) \<omega> (Some (vs @ [v]))"
+    shows "red_pure_exps_total ctxt \<omega>_def es \<omega> (Some vs) \<and> ctxt, \<omega>_def \<turnstile> \<langle>e;\<omega>\<rangle> [\<Down>]\<^sub>t Val v"
+  using assms
+proof (induction es arbitrary: vs)
+  case Nil
+  then show ?case
+    apply (intro conjI)
+    using red_pure_exps_total.simps red_pure_exps_total_singleton
+     apply fastforce
+    using red_exp_list_normal_elim[OF Nil, simplified]
+    by (metis append1_eq_conv append_Nil option.sel red_exp_list_failure_Nil)
+next
+  case (Cons a es)
+  show ?case
+    apply (intro conjI)
+    using Cons
+     apply (smt (z3) Cons_eq_appendI butlast.simps(2) butlast_snoc list.sel(3) list_all2_Cons1 list_all2_Nil2 list_all2_red_pure_exps_total red_pure_exps_total_list_all2)
+    by (smt (verit, ccfv_threshold) Cons.IH Cons.prems append_eq_Cons_conv append_is_Nil_conv list.inject list.simps(3) red_exp_list_normal_elim)
+qed
+
+
+lemma framed_sat_irrelevant_perm_0_locs:
+  assumes "sat ctxt \<omega> mh mp A"
+      and "mh = get_mh_total \<phi>"
+      and "mp = get_mp_total \<phi>"
+      and "assertion_framing_state ctxt StateCons A \<omega>\<^sub>0"
+      and "StateCons (add_to_nm_total_full \<omega>\<^sub>0 (get_nm_total \<phi>))"
+      and "consistent_external ctxt \<phi>"
+      and "differ_only_in_0_perm_locs_hh (add_to_nm_total \<phi> (get_nm_total_full \<omega>\<^sub>0)) hh"
+      and "get_store_total \<omega>\<^sub>0 = get_store_total \<omega>"
+      and "get_hh_total_full \<omega>\<^sub>0 = get_hh_total_full \<omega>"
+      and "get_hh_total_full \<omega> = get_hh_total \<phi>"
+      and "get_hh_total_full \<omega>' = hh"
+      and "get_store_total \<omega>\<^sub>0 = get_store_total \<omega>'"
+      and "supported_pred_body A"
+      and CtxtPredSynWf: "ctxt_pred_syn_wf ctxt"
+      and ConsMono: "mono_prop_downward StateCons"
+    shows "sat ctxt \<omega>' mh mp A"
+  using assms(1-13)
+proof (induction arbitrary: \<phi> \<omega>\<^sub>0 \<omega>' hh rule: sat.inducts)
+  case IH: (SatAcc e_r r e_p p a mh f mp)
+  have "red_pure_exps_total ctxt None [e_r, e_p] \<omega>' (Some [VRef r, VPerm p])"
+    by (rule framed_sat_irrelevant_perm_0_locs_helper(1); (rule IH)?; simp add: IH.hyps(1-2) list_all2_red_pure_exps_total)
+  hence "ctxt, None \<turnstile> \<langle>e_r;\<omega>'\<rangle> [\<Down>]\<^sub>t Val (VRef r)" and "ctxt, None \<turnstile> \<langle>e_p;\<omega>'\<rangle> [\<Down>]\<^sub>t Val (VPerm p)"
+    by (fastforce dest: eval_list_2D)+
+  then show ?case
+    using IH.hyps(3-6)
+    by (blast intro: SatAcc)
+next
+  case IH: (SatAccWildcard e_r r a f mh mp)
+  have "red_pure_exps_total ctxt None [e_r] \<omega>' (Some [VRef r])"
+    by (rule framed_sat_irrelevant_perm_0_locs_helper(1); (rule IH)?; simp add: IH.hyps(1-2) list_all2_red_pure_exps_total)
+  hence "ctxt, None \<turnstile> \<langle>e_r;\<omega>'\<rangle> [\<Down>]\<^sub>t Val (VRef r)"
+    by (fastforce elim: red_exp_list_normal_elim)
+  then show ?case
+    using IH.hyps
+    by (blast intro: SatAccWildcard)
+next
+  case IH: (SatAccPred e_args v_args e_p p mh mp pid pdecl pbody)
+  have "red_pure_exps_total ctxt None (e_args @ [e_p]) \<omega>' (Some (v_args @ [VPerm p]))"
+    by (rule framed_sat_irrelevant_perm_0_locs_helper(1); (rule IH)?; simp add: IH.hyps(1-2) red_pure_exps_append_success)
+  hence "ctxt, None \<turnstile> \<langle>e_p;\<omega>'\<rangle> [\<Down>]\<^sub>t Val (VPerm p)" and "red_pure_exps_total ctxt None e_args \<omega>' (Some v_args)"
+    by (fastforce dest: eval_list_append_to_oneD elim: red_exp_list_normal_elim)+
+  then show ?case
+    using IH.hyps
+    by (blast intro: SatAccPred)
+next
+  case IH: (SatAccPredWildcard e_args v_args mh pid mp pdecl pbody)
+  have "red_pure_exps_total ctxt None e_args \<omega>' (Some v_args)"
+    by (rule framed_sat_irrelevant_perm_0_locs_helper(1); (rule IH)?; simp add: IH.hyps(1-2))
+  then show ?case
+    using IH.hyps
+    by (blast intro: SatAccPredWildcard)
+next
+  case IH: (SatPure e mh mp)
+  have "red_pure_exps_total ctxt None [e] \<omega>' (Some [VBool True])"
+    by (rule framed_sat_irrelevant_perm_0_locs_helper(1); (rule IH)?; simp add: IH.hyps(1-2) list_all2_red_pure_exps_total)
+  then show ?case
+    by (metis IH.hyps(2) IH.hyps(3) SatPure list.discI nth_Cons_0 red_exp_list_normal_elim)
+next
+  case IH: (SatStar mh mh\<^sub>1 mh\<^sub>2 mp mp\<^sub>1 mp\<^sub>2 A B)
+
+  define fnm where fnm: "fnm = get_fnm_total \<phi>"
+  obtain fnm\<^sub>1 where fnm\<^sub>1: "\<And>lp. fnm\<^sub>1 lp = (if mp\<^sub>1 lp = 0 then None else Some (Abs_posreal (mp\<^sub>1 lp), (mp\<^sub>1 lp / mp lp) *\<^sub>s (snd (the (fnm lp)))))"
+    by simp
+  obtain fnm\<^sub>2 where fnm\<^sub>2: "\<And>lp. fnm\<^sub>2 lp = (if mp\<^sub>2 lp = 0 then None else Some (Abs_posreal (mp\<^sub>2 lp), (mp\<^sub>2 lp / mp lp) *\<^sub>s (snd (the (fnm lp)))))"
+    by simp
+  define nm\<^sub>1 where "nm\<^sub>1 = NM mh\<^sub>1 fnm\<^sub>1"
+  define nm\<^sub>2 where "nm\<^sub>2 = NM mh\<^sub>2 fnm\<^sub>2"
+  define \<phi>\<^sub>1 where "\<phi>\<^sub>1 = \<phi>\<lparr> get_nm_total := nm\<^sub>1 \<rparr>"
+  define \<phi>\<^sub>2 where "\<phi>\<^sub>2 = \<phi>\<lparr> get_nm_total := nm\<^sub>2 \<rparr>"
+
+  have "mp\<^sub>1 = get_mp_total \<phi>\<^sub>1"
+    unfolding \<phi>\<^sub>1_def nm\<^sub>1_def
+    apply simp
+    apply standard
+    apply (rename_tac lp)
+    apply (case_tac "fnm\<^sub>1 lp"; cut_tac ?lp=lp in fnm\<^sub>1; simp)
+     apply (metis option.distinct(1))
+    by (metis Abs_posreal_inverse Some_Some_ifD fst_eqD mem_Collect_eq option.inject pperm_pnone_pgt)
+  have "mp\<^sub>2 = get_mp_total \<phi>\<^sub>2"
+    unfolding \<phi>\<^sub>2_def nm\<^sub>2_def
+    apply simp
+    apply standard
+    apply (rename_tac lp)
+    apply (case_tac "fnm\<^sub>2 lp"; cut_tac ?lp=lp in fnm\<^sub>2; simp)
+     apply (metis option.distinct(1))
+    by (metis Abs_posreal_inverse Some_Some_ifD fst_eqD mem_Collect_eq option.inject pperm_pnone_pgt)
+
+  have \<phi>\<^sub>1_extcons: "consistent_external ctxt \<phi>\<^sub>1"
+  proof
+    fix pid vs q nm'
+    assume lpm: "Some (q,nm') = get_fnm_total \<phi>\<^sub>1 (pid,vs)"
+    have "q = Abs_posreal (mp\<^sub>1 (pid,vs))" and
+         "nm' = (mp\<^sub>1 (pid,vs) / mp (pid,vs)) *\<^sub>s (snd (the (fnm (pid,vs))))"
+      using lpm[unfolded \<open>\<phi>\<^sub>1 = _\<close> \<open>nm\<^sub>1 = _\<close>, simplified, simplified fnm\<^sub>1]
+      by (cases "mp\<^sub>1 (pid,vs) = 0"; simp)+
+
+    have "mp (pid,vs) \<ge> mp\<^sub>1 (pid,vs)"
+      by (meson IH.hyps(2) le_funD split_implies_le(1))
+    then obtain q\<^sub>a nm'\<^sub>a where "Some (q\<^sub>a,nm'\<^sub>a) = get_fnm_total \<phi> (pid,vs)"
+      by (metis IH.prems(2) \<open>mp\<^sub>1 = _\<close> get_fnm_total.simps get_mp_0_implies_fnm_None get_mp_total.simps linorder_not_less lpm obtain_lpm_from_mp preal_not_0_gt_0)
+
+    hence extcons\<^sub>a: "consistent_external_wrt_ploc ctxt (\<phi>\<lparr> get_nm_total := nm'\<^sub>a \<rparr>) (pid,vs) (Rep_posreal q\<^sub>a)"
+      by (metis IH.prems(5) consistent_external.cases)
+
+    have the_eq: "snd (the (fnm (pid,vs))) = nm'\<^sub>a"
+      by (metis \<open>Some (q\<^sub>a,nm'\<^sub>a) = _\<close> fnm option.sel sndI)
+
+    have q_pos: "mp\<^sub>1 (pid,vs) > 0"
+      using lpm preal_not_0_gt_0 \<open>mp\<^sub>1 = get_mp_total \<phi>\<^sub>1\<close> get_mp_0_implies_fnm_None
+      by fastforce
+
+    have "Rep_posreal q\<^sub>a = mp (pid,vs)"
+      by (metis IH.prems(2) \<open>Some (q\<^sub>a,nm'\<^sub>a) =_\<close> \<open>mp\<^sub>1 (pid, vs) \<le> mp (pid, vs)\<close> get_fnm_total.simps get_mp_total.simps mem_Collect_eq obtain_lpm_from_mp option.sel order_less_le_trans posreal_to_preal(8) prod.sel(1) q_pos)
+
+    show "consistent_external_wrt_ploc ctxt (\<phi>\<^sub>1\<lparr> get_nm_total := nm' \<rparr>) (pid,vs) (Rep_posreal q)"
+      unfolding \<open>\<phi>\<^sub>1 = _\<close> \<open>nm' = _\<close> the_eq \<open>q = _\<close> Abs_posreal_inverse[of "mp\<^sub>1 (pid,vs)", simplified, OF q_pos]
+      using fraction_consistent_external(1)[OF CtxtPredSynWf extcons\<^sub>a, of "mp\<^sub>1 (pid, vs) / mp (pid, vs)", unfolded \<open>Rep_posreal q\<^sub>a = _\<close>, simplified]
+      apply simp
+      by (metis (mono_tags, lifting) IH.prems(2) \<open>Some (q\<^sub>a,nm'\<^sub>a) = _\<close> get_fnm_total.simps get_mp_0_implies_fnm_None get_mp_total.simps nonzero_eq_divide_eq option.discI preal_to_real(10) preal_to_real(12) preal_to_real(9) zero_preal.abs_eq)
+  qed
+
+  have \<phi>\<^sub>2_extcons: "consistent_external ctxt \<phi>\<^sub>2"
+  proof
+    fix pid vs q nm'
+    assume lpm: "Some (q,nm') = get_fnm_total \<phi>\<^sub>2 (pid,vs)"
+    have "q = Abs_posreal (mp\<^sub>2 (pid,vs))" and
+         "nm' = (mp\<^sub>2 (pid,vs) / mp (pid,vs)) *\<^sub>s (snd (the (fnm (pid,vs))))"
+      using lpm[unfolded \<open>\<phi>\<^sub>2 = _\<close> \<open>nm\<^sub>2 = _\<close>, simplified, simplified fnm\<^sub>2]
+      by (cases "mp\<^sub>2 (pid,vs) = 0"; simp)+
+
+    have "mp (pid,vs) \<ge> mp\<^sub>2 (pid,vs)"
+      by (meson IH.hyps(2) le_funD split_implies_le(2))
+    then obtain q\<^sub>a nm'\<^sub>a where "Some (q\<^sub>a,nm'\<^sub>a) = get_fnm_total \<phi> (pid,vs)"
+      by (metis IH.prems(2) \<open>mp\<^sub>2 = _\<close> get_fnm_total.simps get_mp_0_implies_fnm_None get_mp_total.simps linorder_not_less lpm obtain_lpm_from_mp preal_not_0_gt_0)
+
+    hence extcons\<^sub>a: "consistent_external_wrt_ploc ctxt (\<phi>\<lparr> get_nm_total := nm'\<^sub>a \<rparr>) (pid,vs) (Rep_posreal q\<^sub>a)"
+      by (metis IH.prems(5) consistent_external.cases)
+
+    have the_eq: "snd (the (fnm (pid,vs))) = nm'\<^sub>a"
+      by (metis \<open>Some (q\<^sub>a,nm'\<^sub>a) = _\<close> fnm option.sel sndI)
+
+    have q_pos: "mp\<^sub>2 (pid,vs) > 0"
+      using lpm preal_not_0_gt_0 \<open>mp\<^sub>2 = get_mp_total \<phi>\<^sub>2\<close> get_mp_0_implies_fnm_None
+      by fastforce
+
+    have "Rep_posreal q\<^sub>a = mp (pid,vs)"
+      by (metis IH.prems(2) \<open>Some (q\<^sub>a,nm'\<^sub>a) =_\<close> \<open>mp\<^sub>2 (pid, vs) \<le> mp (pid, vs)\<close> get_fnm_total.simps get_mp_total.simps mem_Collect_eq obtain_lpm_from_mp option.sel order_less_le_trans posreal_to_preal(8) prod.sel(1) q_pos)
+
+    show "consistent_external_wrt_ploc ctxt (\<phi>\<^sub>2\<lparr> get_nm_total := nm' \<rparr>) (pid,vs) (Rep_posreal q)"
+      unfolding \<open>\<phi>\<^sub>2 = _\<close> \<open>nm' = _\<close> the_eq \<open>q = _\<close> Abs_posreal_inverse[of "mp\<^sub>2 (pid,vs)", simplified, OF q_pos]
+      using fraction_consistent_external(1)[OF CtxtPredSynWf extcons\<^sub>a, of "mp\<^sub>2 (pid, vs) / mp (pid, vs)", unfolded \<open>Rep_posreal q\<^sub>a = _\<close>, simplified]
+      apply simp
+      by (metis (mono_tags, lifting) IH.prems(2) \<open>Some (q\<^sub>a,nm'\<^sub>a) = _\<close> get_fnm_total.simps get_mp_0_implies_fnm_None get_mp_total.simps nonzero_eq_divide_eq option.discI preal_to_real(10) preal_to_real(12) preal_to_real(9) zero_preal.abs_eq)
+  qed
+
+  have "nm\<^sub>1 + nm\<^sub>2 = get_nm_total \<phi>"
+    unfolding plus_nested_mask_def nm\<^sub>1_def nm\<^sub>2_def
+    apply simp
+    apply (rule nested_mask_equality)
+    using IH.hyps(1) IH.prems(1)
+     apply auto[1]
+    unfolding fnm[simplified, symmetric]
+    apply simp
+    apply standard
+    apply (rename_tac lp)
+    apply (case_tac "fnm\<^sub>1 lp"; case_tac "fnm\<^sub>2 lp"; simp add: pfun_comb_def)
+    subgoal for lp
+      apply (subgoal_tac "mp lp = 0")
+      apply (metis IH.prems(2) fnm get_fnm_total.simps get_mp_0_implies_fnm_None get_mp_total.simps)
+      apply (subgoal_tac "mp\<^sub>1 lp = 0 \<and> mp\<^sub>2 lp = 0")
+      using IH(2)[simplified, THEN fun_cong, of lp, simplified add_masks_def]
+       apply fastforce
+      using fnm\<^sub>1[of lp] fnm\<^sub>2[of lp]
+      by (metis option.distinct(1))
+    subgoal for lp lpm\<^sub>2
+      apply (subgoal_tac "mp\<^sub>1 lp = 0 \<and> mp\<^sub>2 lp = mp lp \<and> mp\<^sub>2 lp > 0")
+      using fnm\<^sub>2[of lp, simplified]
+       apply (smt (verit, ccfv_SIG) IH.prems(2) PosReal.ppos.rep_eq \<open>get_fnm_nm (get_nm_total \<phi>) = fnm\<close> divide_preal.rep_eq divide_self_if get_mp_total.simps gr_0_is_ppos obtain_lpm_from_mp one_preal.rep_eq option.distinct(1) option.sel preal_semimodule_class.scale_one preal_to_real(12) prod.sel(2))
+      using IH(2)[simplified, THEN fun_cong, of lp, simplified add_masks_def]
+      by (metis add.commute fnm\<^sub>1 fnm\<^sub>2 option.distinct(1) padd_pnone preal_not_0_gt_0)
+    subgoal for lp lpm\<^sub>1
+      apply (subgoal_tac "mp\<^sub>2 lp = 0 \<and> mp\<^sub>1 lp = mp lp \<and> mp\<^sub>1 lp > 0")
+      using fnm\<^sub>2[of lp, simplified]
+       apply (metis IH.prems(2) \<open>get_fnm_nm (get_nm_total \<phi>) = fnm\<close> divide_preal.rep_eq divide_self_if fnm\<^sub>1 get_mp_total.simps obtain_lpm_from_mp one_preal.rep_eq option.distinct(1) option.sel preal_semimodule_class.scale_one preal_to_real(12) prod.sel(2) zero_preal.abs_eq)
+      using IH(2)[simplified, THEN fun_cong, of lp, simplified add_masks_def]
+      by (metis fnm\<^sub>1 fnm\<^sub>2 option.distinct(1) padd_pnone preal_not_0_gt_0)
+    subgoal for lp lpm\<^sub>1 lpm\<^sub>2
+    proof -
+      assume "fnm\<^sub>1 lp = Some lpm\<^sub>1"
+        and "fnm\<^sub>2 lp = Some lpm\<^sub>2"
+      have "Rep_posreal (fst lpm\<^sub>1) = mp\<^sub>1 lp"
+        using \<open>fnm\<^sub>1 lp = Some lpm\<^sub>1\<close> \<open>mp\<^sub>1 = _\<close> nm\<^sub>1_def
+        unfolding \<open>\<phi>\<^sub>1 = _\<close>
+        by auto
+      have "Rep_posreal (fst lpm\<^sub>2) = mp\<^sub>2 lp"
+        using \<open>fnm\<^sub>2 lp = Some lpm\<^sub>2\<close> \<open>mp\<^sub>2 = _\<close> nm\<^sub>2_def
+        unfolding \<open>\<phi>\<^sub>2 = _\<close>
+        by auto
+      have "mp lp > 0"
+        by (metis IH.hyps(2) \<open>fnm\<^sub>1 lp = Some lpm\<^sub>1\<close> fnm\<^sub>1 le_funD option.distinct(1) order_less_imp_not_less order_less_le preal_not_0_gt_0 split_implies_le(1))
+      hence 1: "fnm lp = Some (Abs_posreal (mp lp), snd (the (fnm lp)))"
+        by (metis IH.prems(2) \<open>get_fnm_nm (get_nm_total \<phi>) = fnm\<close> get_mp_total.simps obtain_lpm_from_mp option.sel split_pairs)
+      have 2: "snd lpm\<^sub>1 = (mp\<^sub>1 lp / mp lp) *\<^sub>s snd (the (fnm lp))"
+        by (metis \<open>fnm\<^sub>1 lp = Some lpm\<^sub>1\<close> fnm\<^sub>1 option.discI option.sel split_pairs)
+      have 3: "snd lpm\<^sub>2 = (mp\<^sub>2 lp / mp lp) *\<^sub>s snd (the (fnm lp))"
+        by (metis \<open>fnm\<^sub>2 lp = Some lpm\<^sub>2\<close> fnm\<^sub>2 option.discI option.sel split_pairs)
+      show "Some (fst lpm\<^sub>1 + fst lpm\<^sub>2, nested_mask_merge (snd lpm\<^sub>1) (snd lpm\<^sub>2)) = fnm lp"
+        apply (subst 1)
+        apply standard+
+         apply (rule Rep_posreal_inject[THEN iffD1])
+        unfolding plus_posreal.rep_eq
+         apply (metis Abs_posreal_inject IH.hyps(2) Rep_posreal Rep_posreal_inverse \<open>Rep_posreal (fst lpm\<^sub>1) = mp\<^sub>1 lp\<close> \<open>Rep_posreal (fst lpm\<^sub>2) = mp\<^sub>2 lp\<close> \<open>pos_perm_class.pnone < mp lp\<close> add_masks_def mem_Collect_eq mp_split.simps)
+        unfolding plus_nested_mask_def[symmetric] 2 3
+        unfolding preal_semimodule_class.scale_add_left[symmetric]
+        using preal_semimodule_class.scale_one IH(2)[simplified, THEN fun_cong, of lp, simplified add_masks_def]
+        by (metis PosReal.field_divide_inverse PosReal.field_inverse PosReal.pmult_comm \<open>pos_perm_class.pnone < mp lp\<close> distrib_right preal_not_0_gt_0)
+    qed
+    done
+
+  define \<omega>\<^sub>A where "\<omega>\<^sub>A = add_to_nm_total_full \<omega>\<^sub>0 nm\<^sub>1"
+  have 1: "add_to_nm_total_full \<omega>\<^sub>A nm\<^sub>2 = add_to_nm_total_full \<omega>\<^sub>0 (get_nm_total \<phi>)"
+    apply (rule full_total_state.equality; simp_all add: IH \<omega>\<^sub>A_def)
+    apply (rule total_state.equality; simp_all add: IH \<omega>\<^sub>A_def)
+    using \<open>nm\<^sub>1 + nm\<^sub>2 = _\<close> ab_semigroup_add_class.add_ac(1)
+    by metis
+
+  have "add_to_nm_total_full \<omega>\<^sub>0 (get_nm_total \<phi>) \<succeq> add_to_nm_total_full \<omega>\<^sub>0 nm\<^sub>1"
+    apply (simp add: greater_def)
+    apply (rule exI[of _ "upd_nm_total_full \<omega>\<^sub>0 nm\<^sub>2"])
+    apply (simp add: plus_full_total_state_ext_def plus_total_state_ext_def)
+    apply standard+
+     apply (simp add: \<open>nm\<^sub>1 + nm\<^sub>2 = get_nm_total \<phi>\<close> ab_semigroup_add_class.add_ac(1))
+    by (simp add: defined_def plus_total_state_ext_def)
+
+  hence A_mask_intcons: "StateCons (add_to_nm_total_full \<omega>\<^sub>0 nm\<^sub>1)"
+    using ConsMono IH.prems(4) mono_prop_downwardD
+    by auto
+
+  have *: "add_to_nm_total \<phi>\<^sub>1 (get_nm_total_full \<omega>\<^sub>0) \<le> add_to_nm_total \<phi> (get_nm_total_full \<omega>\<^sub>0)"
+    by (smt (verit) \<open>nm\<^sub>1 + nm\<^sub>2 = get_nm_total \<phi>\<close> \<phi>\<^sub>1_def add_to_nm_total.simps less_eq_total_state_ext_def nm_plus_mono nm_sum_is_bigger total_state.ext_inject total_state.surjective total_state.update_convs(2))
+
+  have **: "add_to_nm_total \<phi>\<^sub>2 (get_nm_total_full \<omega>\<^sub>A) = add_to_nm_total \<phi> (get_nm_total_full \<omega>\<^sub>0)"
+    apply (rule total_state.equality; simp)
+    unfolding \<open>\<phi>\<^sub>2 = _\<close> \<open>\<omega>\<^sub>A = _\<close>
+     apply simp_all
+    by (metis \<open>nm\<^sub>1 + nm\<^sub>2 = get_nm_total \<phi>\<close> add.commute add.left_commute)
+
+  have inhA: "red_inhale ctxt StateCons A \<omega>\<^sub>0 (RNormal (add_to_nm_total_full \<omega>\<^sub>0 nm\<^sub>1))"
+    apply (rule extcons_state_can_be_inhaled_assertion[where hh="get_hh_total \<phi>"])
+               apply fact
+              apply (simp add: nm\<^sub>1_def)
+             apply (simp add: \<open>mp\<^sub>1 = get_mp_total \<phi>\<^sub>1\<close> \<phi>\<^sub>1_def)
+            apply (metis (full_types) \<phi>\<^sub>1_def \<phi>\<^sub>1_extcons old.unit.exhaust total_state.surjective total_state.update_convs(2))
+    using IH.prems(8,9)
+           apply auto[1]
+    using IH.prems(9)
+          apply auto[1]
+         apply (simp add: IH.prems(7))
+    using IH.prems(3) assertion_framing_star
+        apply blast
+    using IH.prems(12)
+       apply force
+    using IH.prems(11)
+      apply auto[1]
+    using A_mask_intcons
+      apply auto[1]
+    by fact+
+
+  show ?case
+    apply (rule SatStar)
+       apply fact
+      apply fact
+     apply (rule IH.IH(1)[where \<phi>=\<phi>\<^sub>1 and \<omega>\<^sub>0=\<omega>\<^sub>0 and hh=hh])
+                apply (simp add: \<phi>\<^sub>1_def nm\<^sub>1_def)
+               apply (simp add: \<open>mp\<^sub>1 = get_mp_total \<phi>\<^sub>1\<close>)
+    using IH.prems(3) assertion_framing_star
+              apply blast
+    using A_mask_intcons \<phi>\<^sub>1_def
+             apply force
+            apply fact
+    using * IH.prems(6) differ_only_in_0_perm_locs_hh_smaller
+           apply blast
+          apply fact+
+    using IH.prems(9) \<open>\<phi>\<^sub>1 = _\<close>
+        apply auto[1]
+    using IH.prems(10)
+       apply auto[1]
+    using IH.prems(11)
+      apply auto[1]
+    using IH.prems(12)
+     apply auto[1]
+    apply (rule IH.IH(2)[where \<phi>=\<phi>\<^sub>2 and \<omega>\<^sub>0=\<omega>\<^sub>A and hh=hh])
+               apply (simp add: \<phi>\<^sub>2_def nm\<^sub>2_def)
+              apply (simp add: \<open>mp\<^sub>2 = get_mp_total \<phi>\<^sub>2\<close>)
+    using IH.prems(3) \<omega>\<^sub>A_def inhA assertion_framing_star
+             apply blast
+    using 1 IH.prems(4) \<phi>\<^sub>2_def
+            apply force
+           apply fact
+    using ** IH.prems(6)
+          apply presburger
+    unfolding \<open>\<omega>\<^sub>A = _\<close>
+         apply (simp add: IH.prems(7))
+    using IH.prems(8)
+        apply auto[1]
+    using IH.prems(9) \<open>\<phi>\<^sub>2 = _\<close>
+       apply auto[1]
+    using IH.prems(10)
+      apply auto[1]
+    using IH.prems(11)
+     apply auto[1]
+    using IH.prems(12)
+    apply auto[1]
+    done
+next
+  case IH: (SatImpTrue e mh mp A)
+  have "red_pure_exps_total ctxt None [e] \<omega>' (Some [VBool True])" and
+       "red_pure_exps_total ctxt (Some \<omega>\<^sub>0) [e] \<omega>\<^sub>0 (Some [VBool True])"
+    by (rule framed_sat_irrelevant_perm_0_locs_helper; (rule IH)?; simp add: IH.hyps(1-2) list_all2_red_pure_exps_total)+
+  hence "ctxt, None \<turnstile> \<langle>e;\<omega>'\<rangle> [\<Down>]\<^sub>t Val (VBool True)" and
+        "ctxt, Some \<omega>\<^sub>0 \<turnstile> \<langle>e;\<omega>\<^sub>0\<rangle> [\<Down>]\<^sub>t Val (VBool True)"
+    by (fastforce elim: red_exp_list_normal_elim)+
+  show ?case
+    apply (rule SatImpTrue)
+     apply fact
+    apply (rule IH.IH[where \<omega>\<^sub>0=\<omega>\<^sub>0])
+               prefer 3
+               apply (rule assertion_framing_imp[OF IH.prems(3)])
+               apply fact
+              apply (rule IH)+
+    using IH.prems(12)
+    by auto
+next
+  case IH: (SatImpFalse e mh mp A)
+  have "red_pure_exps_total ctxt None [e] \<omega>' (Some [VBool False])"
+    by (rule framed_sat_irrelevant_perm_0_locs_helper(1); (rule IH)?; simp add: IH.hyps(1-2) list_all2_red_pure_exps_total)
+  hence "ctxt, None \<turnstile> \<langle>e;\<omega>'\<rangle> [\<Down>]\<^sub>t Val (VBool False)"
+    by (fastforce elim: red_exp_list_normal_elim)
+  show ?case
+    apply (rule SatImpFalse)
+    by fact+
+next
+  case IH: (SatCondTrue e mh mp A B)
+  have "red_pure_exps_total ctxt None [e] \<omega>' (Some [VBool True])" and
+       "red_pure_exps_total ctxt (Some \<omega>\<^sub>0) [e] \<omega>\<^sub>0 (Some [VBool True])"
+    by (rule framed_sat_irrelevant_perm_0_locs_helper; (rule IH)?; simp add: IH.hyps(1-2) list_all2_red_pure_exps_total)+
+  hence "ctxt, None \<turnstile> \<langle>e;\<omega>'\<rangle> [\<Down>]\<^sub>t Val (VBool True)" and
+        "ctxt, Some \<omega>\<^sub>0 \<turnstile> \<langle>e;\<omega>\<^sub>0\<rangle> [\<Down>]\<^sub>t Val (VBool True)"
+    by (fastforce elim: red_exp_list_normal_elim)+
+  show ?case
+    apply (rule SatCondTrue)
+     apply fact
+    apply (rule IH.IH[where \<omega>\<^sub>0=\<omega>\<^sub>0])
+               prefer 3
+               apply (rule assertion_framing_cond_assert_true[OF IH.prems(3)])
+               apply fact
+              apply (rule IH)+
+    using IH.prems(12)
+    by auto
+next
+  case IH: (SatCondFalse e mh mp B A)
+  have "red_pure_exps_total ctxt None [e] \<omega>' (Some [VBool False])" and
+       "red_pure_exps_total ctxt (Some \<omega>\<^sub>0) [e] \<omega>\<^sub>0 (Some [VBool False])"
+    by (rule framed_sat_irrelevant_perm_0_locs_helper; (rule IH)?; simp add: IH.hyps(1-2) list_all2_red_pure_exps_total)+
+  hence "ctxt, None \<turnstile> \<langle>e;\<omega>'\<rangle> [\<Down>]\<^sub>t Val (VBool False)" and
+        "ctxt, Some \<omega>\<^sub>0 \<turnstile> \<langle>e;\<omega>\<^sub>0\<rangle> [\<Down>]\<^sub>t Val (VBool False)"
+    by (fastforce elim: red_exp_list_normal_elim)+
+  show ?case
+    apply (rule SatCondFalse)
+     apply fact
+    apply (rule IH.IH[where \<omega>\<^sub>0=\<omega>\<^sub>0])
+               prefer 3
+               apply (rule assertion_framing_cond_assert_false[OF IH.prems(3)])
+               apply fact
+              apply (rule IH)+
+    using IH.prems(12)
+    by auto
+qed
+
+
+lemma ctxt_pred_self_framing_inh_implies_extcons_irrelevant_perm_0_locs:
+  assumes SFinh: "ctxt_pred_self_framing_inh ctxt StateCons"
+      and ConsMonoSub: "mono_prop_downward_sub_mask_total StateCons_t"
+      and ConsMono: "mono_prop_downward StateCons"
+      and ConsCons_t: "\<forall>\<omega>. StateCons \<omega> \<longleftrightarrow> (StateCons_t (get_total_full \<omega>) \<and> (\<forall>lbl \<phi>. get_trace_total \<omega> lbl = Some \<phi> \<longrightarrow> StateCons_t \<phi>))"
+      and CtxtSynWf: "ctxt_pred_syn_wf ctxt"
+      and "StateCons_t \<phi>"
+      and "differ_only_in_0_perm_locs \<phi> \<phi>'"
+    shows "consistent_external_wrt_ploc ctxt \<phi> (pid,vs) p \<Longrightarrow>
+           consistent_external_wrt_ploc ctxt \<phi>' (pid,vs) p"
+      and "consistent_external ctxt \<phi> \<Longrightarrow>
+           consistent_external ctxt \<phi>'"
+  using assms(6-)
+proof (induction arbitrary: \<phi>' and \<phi>' rule: consistent_external_wrt_ploc_consistent_external.inducts)
+  case IH: (SatStep pid pdecl vs pbody p \<phi>)
+  note diff_only_0_locs = IH.prems(2)[unfolded differ_only_in_0_perm_locs_def]
+  define \<omega>\<^sub>b where "\<omega>\<^sub>b = \<lparr> get_store_total = Map.empty, get_trace_total = Map.empty, get_total_full = \<phi>\<lparr> get_nm_total := 0 \<rparr> \<rparr>"
+  define \<omega>\<^sub>0 where "\<omega>\<^sub>0 = update_store_total \<omega>\<^sub>b (nth_option vs)"
+  show ?case
+    apply (rule SatStep)
+         apply fact+
+    using diff_only_0_locs IH.hyps(2)
+      apply argo
+     apply (rule framed_sat_irrelevant_perm_0_locs[where \<omega>\<^sub>0=\<omega>\<^sub>0 and \<phi>=\<phi> and hh="get_hh_total \<phi>'"])
+    using diff_only_0_locs IH.IH(3)
+                   apply simp
+                  apply (simp add: diff_only_0_locs)
+                 apply (simp add: diff_only_0_locs)
+    unfolding \<open>\<omega>\<^sub>0 = _\<close>
+    using SFinh[unfolded ctxt_pred_self_framing_inh_def
+                assertion_self_framing_def
+                assertion_self_framing_store_def,
+                THEN spec[of _ pid], THEN spec[of _ pdecl], THEN spec[of _ pbody],
+                THEN mp, THEN mp, THEN spec[of _ vs], THEN spec[of _ "Rep_preal p"],
+                THEN mp, THEN spec[of _ \<omega>\<^sub>b]] IH
+                apply blast
+    unfolding \<open>\<omega>\<^sub>b = _\<close>
+               apply simp
+               apply (simp add: ConsCons_t IH.prems(1))
+              apply (simp add: IH.IH(4))
+             apply simp
+    using diff_only_0_locs differ_only_in_0_perm_locs_hh_def
+             apply blast
+            apply simp
+           apply simp
+          apply simp
+         apply simp
+        apply simp
+    using CtxtSynWf IH(1) IH(6) ctxt_pred_syn_wf_def prat_non_negative syntactic_mult_supported
+       apply blast
+      apply (rule CtxtSynWf)
+     apply (rule ConsMono)
+    by (simp add: IH.IH(5) IH.prems(1,2))
+
+next
+  case IH: (SatAll \<phi>)
+  note diff_only_0_locs = IH.prems(2)[unfolded differ_only_in_0_perm_locs_def]
+  show ?case
+    apply (rule SatAll)
+    apply (rule IH(2))
+    using diff_only_0_locs
+      apply simp
+    using ConsMonoSub[unfolded mono_prop_downward_sub_mask_total_def] IH.prems(1) diff_only_0_locs
+     apply simp
+    by (simp add: IH.prems(2) diff_only_0_locs differ_only_in_0_perm_locs_submask)
+qed
+
+
+\<^cancel>\<open>
+lemma inhale_perm_0_locs_irrelevant:
+  assumes "red_inhale ctxt StateCons A \<omega>\<^sub>0 (RNormal \<omega>\<^sub>i)"
+      and "get_store_total \<omega>\<^sub>0 = get_store_total \<omega>\<^sub>0'"
+      and "get_trace_total \<omega>\<^sub>0 = get_trace_total \<omega>\<^sub>0'"
+      and "get_nm_total_full \<omega>\<^sub>0 = get_nm_total_full \<omega>\<^sub>0'"
+      and "get_store_total \<omega>\<^sub>i = get_store_total \<omega>\<^sub>i'"
+      and "get_trace_total \<omega>\<^sub>i = get_trace_total \<omega>\<^sub>i'"
+      and "differ_only_in_0_perm_locs (get_total_full \<omega>\<^sub>i) (get_total_full \<omega>\<^sub>i')"
+      and "get_hh_total_full \<omega>\<^sub>0' = get_hh_total_full \<omega>\<^sub>i'"
+      and ConsHeapIrrelevant:
+            "\<And>\<omega> \<omega>'. get_trace_total \<omega> = get_trace_total \<omega>' \<Longrightarrow>
+                     get_nm_total_full \<omega> = get_nm_total_full \<omega>' \<Longrightarrow>
+                     StateCons \<omega> \<Longrightarrow> StateCons \<omega>'"
+    shows "red_inhale ctxt StateCons A \<omega>\<^sub>0' (RNormal \<omega>\<^sub>i')"
+  using assms(1-8)
+proof (induction A arbitrary: \<omega>\<^sub>0 \<omega>\<^sub>i \<omega>\<^sub>0' \<omega>\<^sub>i')
+  case (Atomic atm)
+  show ?case
+  proof (cases atm)
+    case (Pure e)
+    have "ctxt, Some \<omega>\<^sub>0 \<turnstile> \<langle>e;\<omega>\<^sub>0\<rangle> [\<Down>]\<^sub>t Val (VBool True)" and "\<omega>\<^sub>0 = \<omega>\<^sub>i"
+      using Atomic(1)[unfolded Pure]
+      by (metis InhPure_case result_total.distinct(3) result_total.distinct(5) result_total.inject)+
+    hence "ctxt, Some \<omega>\<^sub>0' \<turnstile> \<langle>e;\<omega>\<^sub>0'\<rangle> [\<Down>]\<^sub>t Val (VBool True)"
+      using eval_perm_0_locs_irrelevant(1)[of \<omega>\<^sub>0 \<omega>\<^sub>0' \<omega>\<^sub>0 \<omega>\<^sub>0']
+      by (metis Atomic.prems(1-4,7,8) differ_only_in_0_perm_locs_smaller extended_val.simps(3) inhale_mono)
+    moreover have "\<omega>\<^sub>0' = \<omega>\<^sub>i'"
+      by (metis (mono_tags) Atomic.prems(2-8) \<open>\<omega>\<^sub>0 = \<omega>\<^sub>i\<close> differ_only_in_0_perm_locs_def full_total_state.surjective get_hh_total_full.simps get_nm_total_full.elims old.unit.exhaust total_state.surjective)
+    ultimately show ?thesis
+      unfolding Pure
+      using red_inhale.InhPure
+      by fastforce
+  next
+    case (Acc e_r f perm)
+    show ?thesis
+    proof (cases perm)
+      case (PureExp e_p)
+      from Atomic(1)[unfolded Acc PureExp] obtain r p W where
+        eval_r: "ctxt, Some \<omega>\<^sub>0 \<turnstile> \<langle>e_r;\<omega>\<^sub>0\<rangle> [\<Down>]\<^sub>t Val (VRef r)" and
+        eval_p: "ctxt, Some \<omega>\<^sub>0 \<turnstile> \<langle>e_p;\<omega>\<^sub>0\<rangle> [\<Down>]\<^sub>t Val (VPerm p)" and
+        "W = (if r = Null then {\<omega>\<^sub>0} else inhale_perm_single StateCons \<omega>\<^sub>0 (the_address r,f) (Some (Abs_preal p)))" and
+        res: "th_result_rel (p \<ge> 0) (W \<noteq> {} \<and> (p > 0 \<longrightarrow> r \<noteq> Null)) W (RNormal \<omega>\<^sub>i)"
+        by (auto elim: InhAcc_case)
+      have "ctxt, Some \<omega>\<^sub>0' \<turnstile> \<langle>e_r;\<omega>\<^sub>0'\<rangle> [\<Down>]\<^sub>t Val (VRef r)"
+        apply (rule eval_perm_0_locs_irrelevant(1)[of \<omega>\<^sub>0 \<omega>\<^sub>0', OF _ _ _ _ _ _ _ _ _ _ eval_r])
+        using Atomic
+                  apply auto
+        by (metis Atomic.prems(4,8) differ_only_in_0_perm_locs_smaller inhale_mono inhale_only_changes_mask)
+      have "ctxt, Some \<omega>\<^sub>0' \<turnstile> \<langle>e_p;\<omega>\<^sub>0'\<rangle> [\<Down>]\<^sub>t Val (VPerm p)"
+        apply (rule eval_perm_0_locs_irrelevant(1)[of \<omega>\<^sub>0 \<omega>\<^sub>0', OF _ _ _ _ _ _ _ _ _ _ eval_p])
+        using Atomic
+                  apply auto
+        by (metis Atomic.prems(4,8) differ_only_in_0_perm_locs_smaller inhale_mono inhale_only_changes_mask)
+
+      define W' where "W' = (if r = Null then {\<omega>\<^sub>0'} else inhale_perm_single StateCons \<omega>\<^sub>0' (the_address r,f) (Some (Abs_preal p)))"
+      have "\<omega>\<^sub>i' \<in> W'"
+        unfolding \<open>W' = _\<close>
+      proof (auto split: if_split)
+        assume "r = Null"
+        hence "\<omega>\<^sub>i = \<omega>\<^sub>0"
+          using \<open>W = _\<close> res th_result_rel_normal
+          by auto
+        thus "\<omega>\<^sub>i' = \<omega>\<^sub>0'"
+          by (metis (mono_tags) Atomic.prems(2-8) differ_only_in_0_perm_locs_def full_total_state.equality get_hh_total_full.simps get_nm_total_full.simps old.unit.exhaust total_state.surjective)
+      next
+        assume "r \<noteq> Null"
+        hence "\<omega>\<^sub>i \<in> inhale_perm_single StateCons \<omega>\<^sub>0 (the_address r, f) (Some (Abs_preal p))"
+          using \<open>W = _\<close> res th_result_rel_normal
+          by auto
+        hence "\<omega>\<^sub>i = upd_mh_loc_total_full \<omega>\<^sub>0 (the_address r, f) (get_mh_total_full \<omega>\<^sub>0 (the_address r, f) + Abs_preal p)"
+          unfolding inhale_perm_single_def
+          by fastforce
+        show "\<omega>\<^sub>i' \<in> inhale_perm_single StateCons \<omega>\<^sub>0' (the_address r, f) (Some (Abs_preal p))"
+          unfolding inhale_perm_single_def
+          apply (rule CollectI)
+          apply (rule exI[of _ \<omega>\<^sub>i'])
+          apply (rule exI[of _ "Abs_preal p"])
+          apply (intro conjI)
+             apply simp
+            apply simp
+           apply (rule full_total_state.equality)
+              prefer 4
+          using inhale_only_changes_mask[OF Atomic(1)] Atomic
+              apply (simp, simp, simp)
+           apply (rule total_state.equality)
+             prefer 3
+          using inhale_only_changes_mask[OF Atomic(1)] Atomic
+             apply (simp, simp)
+          using \<open>\<omega>\<^sub>i = _\<close> Atomic
+           apply (simp add: differ_only_in_0_perm_locs_def)
+          apply (rule ConsHeapIrrelevant[of \<omega>\<^sub>i])
+          using Atomic Atomic(7)[unfolded differ_only_in_0_perm_locs_def] \<open>\<omega>\<^sub>i \<in> _\<close>[unfolded inhale_perm_single_def]
+          by auto
+      qed
+
+      show ?thesis
+        unfolding Acc PureExp
+        apply (rule InhAcc)
+           apply fact+
+        by (metis (full_types) THResultNormal_alt \<open>\<omega>\<^sub>i' \<in> W'\<close> res all_not_in_conv th_result_rel_normal)
+    next
+      case Wildcard
+      from Atomic(1)[unfolded Acc Wildcard] obtain r W where
+        eval_r: "ctxt, Some \<omega>\<^sub>0 \<turnstile> \<langle>e_r;\<omega>\<^sub>0\<rangle> [\<Down>]\<^sub>t Val (VRef r)" and
+        "W = inhale_perm_single StateCons \<omega>\<^sub>0 (the_address r,f) None" and
+        res: "th_result_rel True (W \<noteq> {} \<and> r \<noteq> Null) W (RNormal \<omega>\<^sub>i)"
+        by (auto elim: InhAccWildcard_case)
+      have "ctxt, Some \<omega>\<^sub>0' \<turnstile> \<langle>e_r;\<omega>\<^sub>0'\<rangle> [\<Down>]\<^sub>t Val (VRef r)"
+        apply (rule eval_perm_0_locs_irrelevant(1)[of \<omega>\<^sub>0 \<omega>\<^sub>0', OF _ _ _ _ _ _ _ _ _ _ eval_r])
+        using Atomic
+                  apply auto
+        by (metis Atomic.prems(4,8) differ_only_in_0_perm_locs_smaller inhale_mono inhale_only_changes_mask)
+
+      define W' where "W' = inhale_perm_single StateCons \<omega>\<^sub>0' (the_address r,f) None"
+      have "\<omega>\<^sub>i' \<in> W'"
+        unfolding \<open>W' = _\<close>
+      proof -
+        have "\<omega>\<^sub>i \<in> inhale_perm_single StateCons \<omega>\<^sub>0 (the_address r, f) None"
+          using \<open>W = _\<close> res th_result_rel_normal
+          by auto
+        then obtain q where
+          "option_fold ((=) q) (q \<noteq> 0) None" and
+          "\<omega>\<^sub>i = upd_mh_loc_total_full \<omega>\<^sub>0 (the_address r, f) (get_mh_total_full \<omega>\<^sub>0 (the_address r, f) + q)" and
+          "StateCons \<omega>\<^sub>i"
+          using inhale_perm_single_def
+          by blast
+        show "\<omega>\<^sub>i' \<in> inhale_perm_single StateCons \<omega>\<^sub>0' (the_address r, f) None"
+          unfolding inhale_perm_single_def
+          apply (rule CollectI)
+          apply (rule exI[of _ \<omega>\<^sub>i'])
+          apply (rule exI[of _ q])
+          apply (intro conjI)
+             apply simp
+            apply fact
+           apply (rule full_total_state.equality)
+              prefer 4
+          using inhale_only_changes_mask[OF Atomic(1)] Atomic
+              apply (simp, simp, simp)
+           apply (rule total_state.equality)
+             prefer 3
+          using inhale_only_changes_mask[OF Atomic(1)] Atomic
+             apply (simp, simp)
+          using \<open>\<omega>\<^sub>i = _\<close> Atomic
+           apply (simp add: differ_only_in_0_perm_locs_def)
+          apply (rule ConsHeapIrrelevant[of \<omega>\<^sub>i])
+          using Atomic Atomic(7)[unfolded differ_only_in_0_perm_locs_def] \<open>\<omega>\<^sub>i \<in> _\<close>[unfolded inhale_perm_single_def]
+          by auto
+      qed
+
+      show ?thesis
+        unfolding Acc Wildcard
+        apply (rule InhAccWildcard)
+          apply fact+
+        by (metis (mono_tags, opaque_lifting) THResultNormal_alt \<open>\<omega>\<^sub>i' \<in> W'\<close> emptyE res th_result_rel_normal)
+    qed
+  next
+    case (AccPredicate pid e_args perm)
+    show ?thesis
+    proof (cases perm)
+      case (PureExp e_p)
+      from Atomic(1)[unfolded AccPredicate PureExp] obtain vs p W where
+        eval_vs: "red_pure_exps_total ctxt (Some \<omega>\<^sub>0) e_args \<omega>\<^sub>0 (Some vs)" and
+        eval_p: "ctxt, Some \<omega>\<^sub>0 \<turnstile> \<langle>e_p;\<omega>\<^sub>0\<rangle> [\<Down>]\<^sub>t Val (VPerm p)" and
+        "W = inhale_perm_single_pred ctxt StateCons \<omega>\<^sub>0 (pid,vs) (Some (Abs_preal p))" and
+        res: "th_result_rel (p \<ge> 0) (W \<noteq> {}) W (RNormal \<omega>\<^sub>i)"
+        by (auto elim: InhAccPredPerm_case)
+      have "red_pure_exps_total ctxt (Some \<omega>\<^sub>0') e_args \<omega>\<^sub>0' (Some vs)"
+        apply (rule eval_perm_0_locs_irrelevant(2)[of \<omega>\<^sub>0 \<omega>\<^sub>0', OF _ _ _ _ _ _ _ _ _ _ eval_vs])
+        using Atomic
+                  apply auto
+        by (metis Atomic.prems(4,8) differ_only_in_0_perm_locs_smaller inhale_mono inhale_only_changes_mask)
+      have "ctxt, Some \<omega>\<^sub>0' \<turnstile> \<langle>e_p;\<omega>\<^sub>0'\<rangle> [\<Down>]\<^sub>t Val (VPerm p)"
+        apply (rule eval_perm_0_locs_irrelevant(1)[of \<omega>\<^sub>0 \<omega>\<^sub>0', OF _ _ _ _ _ _ _ _ _ _ eval_p])
+        using Atomic
+                  apply auto
+        by (metis Atomic.prems(4,8) differ_only_in_0_perm_locs_smaller inhale_mono inhale_only_changes_mask)
+
+      define W' where "W' = inhale_perm_single_pred ctxt StateCons \<omega>\<^sub>0' (pid,vs) (Some (Abs_preal p))"
+      have "\<omega>\<^sub>i' \<in> W'"
+        unfolding \<open>W' = _\<close>
+      proof -
+        have "\<omega>\<^sub>i \<in> inhale_perm_single_pred ctxt StateCons \<omega>\<^sub>0 (pid,vs) (Some (Abs_preal p))"
+          using \<open>W = _\<close> res th_result_rel_normal
+          by auto
+        then obtain q \<phi>_inh where
+          "option_fold ((=) q) (q \<noteq> 0) (Some (Abs_preal p))" and
+          "consistent_external_wrt_ploc ctxt \<phi>_inh (pid,vs) q" and
+          \<phi>_inh_hh: "get_hh_total \<phi>_inh = get_hh_total_full \<omega>\<^sub>0" and
+          "\<omega>\<^sub>i = (if q = 0 then \<omega>\<^sub>0 else add_to_lpm_nonzero_total_full \<omega>\<^sub>0 (pid,vs) (Abs_posreal q) (get_nm_total \<phi>_inh))"
+          "StateCons \<omega>\<^sub>i"
+          using inhale_perm_single_pred_def
+          by blast
+        show "\<omega>\<^sub>i' \<in> inhale_perm_single_pred ctxt StateCons \<omega>\<^sub>0' (pid,vs) (Some (Abs_preal p))"
+          unfolding inhale_perm_single_pred_def
+          apply (rule CollectI)
+          apply (rule exI[of _ \<omega>\<^sub>i'])
+          apply (rule exI[of _ "\<phi>_inh\<lparr> get_hh_total := get_hh_total_full \<omega>\<^sub>0' \<rparr>"])
+          apply (rule exI[of _ q])
+          apply (intro conjI)
+               apply simp
+              apply fact
+            (* unprovable *)
+          done
+      qed
+
+      show ?thesis
+        unfolding AccPredicate PureExp
+        apply (rule InhAccPred)
+          apply fact+
+        by (metis (mono_tags, opaque_lifting) THResultNormal_alt \<open>\<omega>\<^sub>i' \<in> W'\<close> emptyE res th_result_rel_normal)
+    next
+      case Wildcard
+      then show ?thesis done
+    qed
+  qed
+
+next
+  case IH: (Imp e A)
+
+  have "\<omega>\<^sub>0 \<le> \<omega>\<^sub>i"
+    using IH.prems(1) inhale_mono
+    by blast
+  hence diff_only_0_locs: "differ_only_in_0_perm_locs (get_total_full \<omega>\<^sub>0) (get_total_full \<omega>\<^sub>0')"
+    using IH.prems(4,7,8) differ_only_in_0_perm_locs_smaller less_eq_full_total_stateD_2
+    by blast
+
+  from IH consider (True) "ctxt, Some \<omega>\<^sub>0 \<turnstile> \<langle>e;\<omega>\<^sub>0\<rangle> [\<Down>]\<^sub>t Val (VBool True)" |
+                  (False) "ctxt, Some \<omega>\<^sub>0 \<turnstile> \<langle>e;\<omega>\<^sub>0\<rangle> [\<Down>]\<^sub>t Val (VBool False)"
+    by (auto elim: InhImp_case)
+  then show ?case
+  proof cases
+    case True
+    hence *: "red_inhale ctxt StateCons A \<omega>\<^sub>0 (RNormal \<omega>\<^sub>i)"
+      by (metis IH.prems(1) InhImp_case ValueAndBasicState.val.inject(2) eval_is_deterministic_single extended_val.inject result_total.distinct(5))
+    show ?thesis
+      apply (rule InhImpTrue)
+       apply (metis IH.prems(2-4) True diff_only_0_locs eval_perm_0_locs_irrelevant(1) extended_val.distinct(1))
+      apply (rule IH(1))
+             apply (rule *)
+      using IH
+      by auto
+  next
+    case False
+    hence "\<omega>\<^sub>i = \<omega>\<^sub>0"
+      by (metis (full_types) IH.prems(1) InhImp_case ValueAndBasicState.val.inject(2) eval_is_deterministic_single extended_val.inject result_total.distinct(5) result_total.inject)
+    show ?thesis
+      apply (rule InhImpFalse)
+       apply (metis False IH.prems(2-4) diff_only_0_locs eval_perm_0_locs_irrelevant(1) extended_val.distinct(1))
+      using IH \<open>\<omega>\<^sub>i = \<omega>\<^sub>0\<close>
+      by (simp add: differ_only_in_0_perm_locs_def)
+  qed
+
+next
+  case IH: (CondAssert e A B)
+
+  have "\<omega>\<^sub>0 \<le> \<omega>\<^sub>i"
+    using IH.prems(1) inhale_mono
+    by blast
+  hence diff_only_0_locs: "differ_only_in_0_perm_locs (get_total_full \<omega>\<^sub>0) (get_total_full \<omega>\<^sub>0')"
+    using IH.prems(4,7,8) differ_only_in_0_perm_locs_smaller less_eq_full_total_stateD_2
+    by blast
+
+  from IH consider (True) "ctxt, Some \<omega>\<^sub>0 \<turnstile> \<langle>e;\<omega>\<^sub>0\<rangle> [\<Down>]\<^sub>t Val (VBool True)" |
+                  (False) "ctxt, Some \<omega>\<^sub>0 \<turnstile> \<langle>e;\<omega>\<^sub>0\<rangle> [\<Down>]\<^sub>t Val (VBool False)"
+    by (auto elim: red_inhale.cases)
+  then show ?case
+  proof cases
+    case True
+    hence *: "red_inhale ctxt StateCons A \<omega>\<^sub>0 (RNormal \<omega>\<^sub>i)"
+      by (metis IH.prems(1) InhCondAssert ValueAndBasicState.val.inject(2) eval_is_deterministic_single extended_val.inject result_total.simps(7))
+    show ?thesis
+      apply (rule InhCondAssertTrue)
+       apply (metis IH.prems(2-4) True diff_only_0_locs eval_perm_0_locs_irrelevant(1) extended_val.distinct(1))
+      apply (rule IH(1))
+             apply (rule *)
+      using IH
+      by auto
+  next
+    case False
+    hence *: "red_inhale ctxt StateCons B \<omega>\<^sub>0 (RNormal \<omega>\<^sub>i)"
+      by (metis IH.prems(1) InhCondAssert ValueAndBasicState.val.inject(2) eval_is_deterministic_single extended_val.inject result_total.simps(7))
+    show ?thesis
+      apply (rule InhCondAssertFalse)
+       apply (metis IH.prems(2-4) False diff_only_0_locs eval_perm_0_locs_irrelevant(1) extended_val.distinct(1))
+      apply (rule IH(2))
+             apply (rule *)
+      using IH
+      by auto
+  qed
+
+next
+  case IH: (Star A B)
+  then obtain \<omega>'' where
+    inhA: "red_inhale ctxt StateCons A \<omega>\<^sub>0 (RNormal \<omega>'')" and
+    inhB: "red_inhale ctxt StateCons B \<omega>'' (RNormal \<omega>\<^sub>i)"
+    by (blast elim: InhStar_case)
+  define \<omega>''' where "\<omega>''' = upd_hh_total_full \<omega>'' (get_hh_total_full \<omega>\<^sub>0')"
+  hence "\<omega>'' \<le> \<omega>\<^sub>i"
+    using inhB
+    by (simp add: inhale_mono)
+  have "differ_only_in_0_perm_locs (get_total_full \<omega>'') (get_total_full \<omega>''')"
+    apply (rule differ_only_in_0_perm_locs_smaller[OF IH(9)])
+    unfolding \<open>\<omega>''' = _\<close>
+       apply simp
+    using \<open>\<omega>'' \<le> \<omega>\<^sub>i\<close> less_eq_full_total_stateD_2
+      apply blast
+     apply simp
+    using IH.prems(8)
+     apply auto[1]
+    by fact
+
+  show ?case
+    apply (rule InhStarNormal)
+     apply (rule IH(1)[OF inhA, of \<omega>\<^sub>0' "\<omega>'''"])
+           apply (simp add: IH.prems(2))
+          apply (simp add: IH.prems(3))
+    using IH.prems(4)
+         apply auto[1]
+        apply (simp add: \<open>\<omega>''' = _\<close>)
+       apply (simp add: \<open>\<omega>''' = _\<close>)
+      apply fact
+     apply (simp add: \<open>\<omega>''' = _\<close>)
+    apply (rule IH(2)[OF inhB])
+          apply (simp add: \<open>\<omega>''' = _\<close>)
+         apply (simp add: \<open>\<omega>''' = _\<close>)
+        apply (simp add: \<open>\<omega>''' = _\<close>)
+       apply fact
+      apply fact
+     apply fact
+    unfolding \<open>\<omega>''' = _\<close>
+    apply simp
+    using IH.prems(8)
+    by auto
+qed (auto elim: red_inhale.cases)
+\<close>
+
+
+\<comment> \<open>Unused\<close>
+lemma inhale_sat:
+  assumes "red_inhale ctxt StateCons A \<omega> (RNormal \<omega>')"
+      and "(\<lambda>l. get_mh_total_full \<omega> l + mh l) = get_mh_total_full \<omega>'"
+      and "(\<lambda>l. get_mp_total_full \<omega> l + mp l) = get_mp_total_full \<omega>'"
+    shows "sat ctxt \<omega> mh mp A"
   oops
+
+
+lemma ctxt_pred_self_framing_inh_implies_sat:
+  assumes CtxtPredSynWf: "ctxt_pred_syn_wf ctxt"
+      and ConsMonoSub: "mono_prop_downward_sub_mask_total StateCons_t"
+      and MonoCons: "mono_prop_downward StateCons"
+      and ConsCons_t: "\<forall>\<omega>. StateCons \<omega> \<longleftrightarrow> (StateCons_t (get_total_full \<omega>) \<and> (\<forall>lbl \<phi>. get_trace_total \<omega> lbl = Some \<phi> \<longrightarrow> StateCons_t \<phi>))"
+      and CtxtPredSFinh: "ctxt_pred_self_framing_inh ctxt StateCons"
+    shows "ctxt_pred_self_framing_sat ctxt StateCons_t"
+  unfolding ctxt_pred_self_framing_sat_def pred_self_framing_def
+  using ConsCons_t ConsMonoSub CtxtPredSFinh CtxtPredSynWf MonoCons ctxt_pred_self_framing_inh_implies_extcons_irrelevant_perm_0_locs(1)
+  by blast
+
 
 
 end
